poSTVM/poSTVM_state_alt.thy
@@ -20,45 +20,56 @@ type_synonym program_context ="stacked_prog_vars *
                              ((process_name,process_context) fmap) * 
                              process_name"
 
-text "Model state in form of global vars, programs map, current program, function blocks list, functions list"
-datatype model_context = ST 
-                       stacked_global_vars  
-                       "(program_name,program_context) fmap" 
-                       program_name 
-                       stacked_func_blocks  
-                       stacked_funcs
+text "Model state in form of global vars, programs map, current program, function blocks list, functions list, last value"
+type_synonym model_context =
+"stacked_global_vars * ((program_name,program_context) fmap) *
+program_name * stacked_func_blocks * stacked_funcs * ptype"
 
 datatype var_level = Global | Program | Process
 
+text "Getting last model value"
+definition get_value :: "model_context \<Rightarrow> ptype" where
+"get_value st = (let (g1, pg_map, pg_name, f1, f2, value) = st in value)"
+declare get_value_def [simp]
+
+text "Setting last model value"
+definition set_value :: "model_context \<Rightarrow> ptype \<Rightarrow> model_context" where
+"set_value st val = (let (g2, pg_map, pg_name, f1, f2, value) = st in (g2, pg_map, pg_name, f1, f2, val))"
+declare set_value_def [simp]
+
 text "Getting var init from process vars by name"
-definition get_proc_var_by_name :: "stacked_proc_vars \<Rightarrow>  symbolic_var \<Rightarrow>  stacked_var_init option" where
+definition get_proc_var_by_name :: "stacked_proc_vars \<Rightarrow>  symbolic_var \<Rightarrow>  stacked_var_init " where
   "get_proc_var_by_name vars name =
     (case the (fmlookup vars name) of
-      (stacked_proc_var.Var var) \<Rightarrow> Some var
-    | (stacked_proc_var.InOutVar var) \<Rightarrow> Some var
-    | (stacked_proc_var.InVar var) \<Rightarrow> Some var
-    | (stacked_proc_var.OutVar var) \<Rightarrow> Some var
-    | (stacked_proc_var.ProcessVar var) \<Rightarrow> None)"
+      (stacked_proc_var.Var var) \<Rightarrow> var
+    | (stacked_proc_var.InOutVar var) \<Rightarrow> var
+    | (stacked_proc_var.InVar var) \<Rightarrow> var
+    | (stacked_proc_var.OutVar var) \<Rightarrow> var)"
 declare get_proc_var_by_name_def [simp]
+(*
+    | (stacked_proc_var.ProcessVar var) \<Rightarrow> None
+*)
 
 text "Getting var init from program vars by name"
-definition get_prog_var_by_name :: "stacked_prog_vars \<Rightarrow>  symbolic_var \<Rightarrow>  stacked_var_init option" where
+definition get_prog_var_by_name :: "stacked_prog_vars \<Rightarrow>  symbolic_var \<Rightarrow>  stacked_var_init" where
   "get_prog_var_by_name vars name =
     (case the (fmlookup vars name) of
-      (stacked_prog_var.Var var) \<Rightarrow> Some var
-    | (stacked_prog_var.InOutVar var) \<Rightarrow> Some var
-    | (stacked_prog_var.InVar var) \<Rightarrow> Some var
-    | (stacked_prog_var.OutVar var) \<Rightarrow> Some var
-    | (stacked_prog_var.ExtVar var) \<Rightarrow>Some var)"
+      (stacked_prog_var.Var var) \<Rightarrow> var
+    | (stacked_prog_var.InOutVar var) \<Rightarrow> var
+    | (stacked_prog_var.InVar var) \<Rightarrow> var
+    | (stacked_prog_var.OutVar var) \<Rightarrow> var
+    | (stacked_prog_var.ExtVar var) \<Rightarrow> var)"
 declare get_prog_var_by_name_def [simp]
 
 text "Getting var init from global vars by name"
-definition get_global_var_by_name :: "stacked_global_vars \<Rightarrow>  symbolic_var \<Rightarrow>  stacked_var_init option" where
-  "get_global_var_by_name vars name =
+definition get_var_from_global_vars_by_name :: "stacked_global_vars \<Rightarrow>  symbolic_var \<Rightarrow>  stacked_var_init" where
+ "get_var_from_global_vars_by_name vars name =
     (case the (fmlookup vars name) of
-      (stacked_global_var.Var var) \<Rightarrow> Some var
-    | (stacked_global_var.Global _ var) \<Rightarrow> None)"
-declare get_global_var_by_name_def [simp]
+      (stacked_global_var.Var var) \<Rightarrow> var
+)"
+declare get_var_from_global_vars_by_name_def [simp]
+(*| (stacked_global_var.Global _ var) \<Rightarrow> var*)
+
 
 print_theorems
 
@@ -82,10 +93,9 @@ declare get_cur_proc_vars_from_progst_def [simp]
 text "Getting current program state from model state"
 definition get_cur_progst :: "model_context \<Rightarrow> program_context" where
 "get_cur_progst st = 
-  (case st of 
-    (ST global_var_decl_list ps_map p_name function_block_decl_list function_decl_list) \<Rightarrow>
-      (case (fmlookup ps_map p_name) of 
-        Some(p_state) \<Rightarrow> p_state))"
+  (let (global_var_list, pg_map, pg_name, function_block_list, function_list, value) = st in
+    (case (fmlookup pg_map pg_name) of 
+        Some(ps_state) \<Rightarrow> ps_state))"
 declare get_cur_progst_def [simp]
 
 text "Getting current process state name"
@@ -111,9 +121,39 @@ declare get_cur_prog_vars_def [simp]
 
 text "Get global vars"
 definition get_global_vars :: "model_context \<Rightarrow> stacked_global_vars" where
-"get_global_vars st = (case st of (ST vars _ _ _ _) \<Rightarrow> vars)"
+"get_global_vars st = 
+(let (global_var_list, pg_map, pg_name, function_block_list, function_list, value) = st in
+  global_var_list)"
 declare get_global_vars_def [simp]
 
+text "Setting global vars in model context"
+definition set_global_vars :: "model_context \<Rightarrow> stacked_global_vars \<Rightarrow> model_context" where
+"set_global_vars st vars = (let (_, pg_map, pg_name, f1, f2, v) = st in (vars, pg_map, pg_name, f1, f2, v))"
+declare set_global_vars_def [simp]
+
+text "Checking if var with given name exists"
+definition var_exists :: "model_context \<Rightarrow> symbolic_var \<Rightarrow> bool" where
+"var_exists st var_name =
+  (case (fmlookup (get_global_vars st) var_name) of
+    Some _ \<Rightarrow> True
+  | None \<Rightarrow> (case (fmlookup (get_cur_prog_vars st) var_name) of
+              Some _ \<Rightarrow> True
+            | None \<Rightarrow> (case (fmlookup (get_cur_proc_vars st) var_name) of
+                        Some _ \<Rightarrow> True
+                      | None \<Rightarrow> False)))"
+declare var_exists_def [simp]
+
+text "Getting level of var by name"
+definition get_var_level_by_name :: "model_context \<Rightarrow> symbolic_var \<Rightarrow> var_level" where
+"get_var_level_by_name st var_name =
+  (case (fmlookup (get_global_vars st) var_name) of
+    Some _ \<Rightarrow> var_level.Global
+  | None \<Rightarrow> (case (fmlookup (get_cur_prog_vars st) var_name) of
+              Some _ \<Rightarrow> var_level.Program
+            | None \<Rightarrow> (case (fmlookup (get_cur_proc_vars st) var_name) of
+                        Some _ \<Rightarrow> var_level.Process)))"
+declare get_var_level_by_name_def [simp]
+(*
 text "Getting level of var by name for setting purpose"
 definition get_var_level_by_name_for_set :: "model_context \<Rightarrow> symbolic_var \<Rightarrow> var_level" where
 "get_var_level_by_name_for_set st var_name =
@@ -135,382 +175,399 @@ definition get_var_level_by_name_for_get :: "model_context \<Rightarrow> symboli
             | None \<Rightarrow> (case (fmlookup (get_cur_proc_vars st) var_name) of
                         Some _ \<Rightarrow> var_level.Process)))"
 declare get_var_level_by_name_for_get_def [simp]
-
+*)
 text "Getting variable init by name from model state"
 definition get_cur_var_init_by_name :: "model_context \<Rightarrow> symbolic_var \<Rightarrow> stacked_var_init" where
 "get_cur_var_init_by_name st var_name = 
-  (case (get_var_level_by_name_for_get st var_name) of
-    var_level.Global \<Rightarrow> the (get_global_var_by_name (get_global_vars st) var_name)
-  | var_level.Program \<Rightarrow> the (get_prog_var_by_name (get_cur_prog_vars st) var_name)
-  | var_level.Process \<Rightarrow> the (get_proc_var_by_name (get_cur_proc_vars st) var_name))"
+  (case (get_var_level_by_name st var_name) of
+    var_level.Global \<Rightarrow> (get_var_from_global_vars_by_name (get_global_vars st) var_name)
+  | var_level.Program \<Rightarrow> (get_prog_var_by_name (get_cur_prog_vars st) var_name)
+  | var_level.Process \<Rightarrow> (get_proc_var_by_name (get_cur_proc_vars st) var_name))"
 declare get_cur_var_init_by_name_def [simp]
 
 text "Getting symbolic variable value by name from model state"
-definition get_cur_symbvar_by_name :: "model_context \<Rightarrow> symbolic_var \<Rightarrow> basic_post_type" where
+definition get_cur_symbvar_by_name :: "model_context \<Rightarrow> symbolic_var \<Rightarrow> ptype" where
 "get_cur_symbvar_by_name st var_name = 
   (case (get_cur_var_init_by_name st var_name) of
     (stacked_var_init.Symbolic val opt) \<Rightarrow> val)"
 declare get_cur_symbvar_by_name_def [simp]
 
-text "Getting value from list of values by basic_post_type position"
-definition get_val_from_list_by_basic :: "'a list \<Rightarrow> basic_post_type \<Rightarrow> 'a" where
+text "Getting value from list of values by ptype position"
+definition get_val_from_list_by_basic :: "'a list \<Rightarrow> ptype \<Rightarrow> 'a" where
 "get_val_from_list_by_basic bl pos =
   (case pos of
-    (basic_post_type.Nat val) \<Rightarrow> (nth bl val) |
-    (basic_post_type.Int val) \<Rightarrow> (nth bl (nat val)))"
+    (ptype.Nat val) \<Rightarrow> (nth bl val) |
+    (ptype.Int val) \<Rightarrow> (nth bl (nat val)))"
 declare get_val_from_list_by_basic_def [simp]
 
 text "Getting array variable single values by name and absolute position from model state"
-definition get_cur_arvar_by_name_by_pos :: "model_context \<Rightarrow> symbolic_var \<Rightarrow> basic_post_type \<Rightarrow> basic_post_type" where
+definition get_cur_arvar_by_name_by_pos :: "model_context \<Rightarrow> symbolic_var \<Rightarrow> ptype \<Rightarrow> ptype" where
 "get_cur_arvar_by_name_by_pos st var_name pos =
   (case (get_cur_var_init_by_name st var_name) of
     (stacked_var_init.Array (stacked_array_interval.Int val1 val2) values  opt) \<Rightarrow>
-      (get_val_from_list_by_basic values (basic_post_type_sum (basic_post_type.Int val1) pos)))"
+      (get_val_from_list_by_basic values (ptype_sum (ptype.Int val1) pos)))"
 declare get_cur_arvar_by_name_by_pos_def [simp]
 
 text "Setting in process vars list new var init value by name"
-definition set_symbvar_in_proc_vars :: "(stacked_proc_vars) \<Rightarrow>  symbolic_var \<Rightarrow> stacked_var_init \<Rightarrow> stacked_proc_vars" where
-"set_symbvar_in_proc_vars vars name val= 
+definition set_cur_symbvar_in_proc_vars :: "(stacked_proc_vars) \<Rightarrow>  symbolic_var \<Rightarrow> stacked_var_init \<Rightarrow> stacked_proc_vars" where
+"set_cur_symbvar_in_proc_vars vars name val= 
   (case the (fmlookup vars name) of
     (stacked_proc_var.Var var) \<Rightarrow> (fmupd name (stacked_proc_var.Var val) vars)
   | (stacked_proc_var.InOutVar var) \<Rightarrow> (fmupd name (stacked_proc_var.InOutVar val) vars)
   | (stacked_proc_var.InVar var) \<Rightarrow> (fmupd name (stacked_proc_var.InVar val) vars)
   | (stacked_proc_var.OutVar var) \<Rightarrow> (fmupd name (stacked_proc_var.OutVar val) vars))"
-declare set_symbvar_in_proc_vars_def [simp]
+declare set_cur_symbvar_in_proc_vars_def [simp]
 
 text "Setting symbolic var in current process in model state"
-definition set_cur_proc_symbvar :: "model_context \<Rightarrow> symbolic_var \<Rightarrow> stacked_var_init \<Rightarrow> model_context" where
-"set_cur_proc_symbvar st var_name val = 
-  (case st of (ST global_vars pg_map pg_name  f1 f2) \<Rightarrow>
-    (let (prog_vars,pc_map,pc_name) = the (fmlookup pg_map pg_name);
-         (proc_vars,v1,v2,v3,v4,v5) = the (fmlookup pc_map pc_name)
-     in (ST
-         global_vars 
+definition set_cur_proc_var :: "model_context \<Rightarrow> symbolic_var \<Rightarrow> stacked_var_init \<Rightarrow> model_context" where
+"set_cur_proc_var st var_name val = 
+  (let (global_vars, pg_map, pg_name, f1, f2, value) = st; 
+      (prog_vars,pc_map,pc_name) = the (fmlookup pg_map pg_name);
+      (proc_vars,v1,v2,v3,v4,v5) = the (fmlookup pc_map pc_name)
+     in (global_vars, 
          (fmupd
           pg_name
           (prog_vars,
            (fmupd
             pc_name
-            (set_symbvar_in_proc_vars proc_vars var_name val,v1,v2,v3,v4,v5)
+            (set_cur_symbvar_in_proc_vars proc_vars var_name val,v1,v2,v3,v4,v5)
             pc_map),
            pc_name)
-          pg_map)
-          pg_name
-         f1
-         f2)))"
-declare set_cur_proc_symbvar_def [simp]
+          pg_map),
+          pg_name,
+         f1,
+         f2,
+         value))"
+declare set_cur_proc_var_def [simp]
 
 text "Setting symbolic var in program vars"
-definition set_symbvar_in_prog_vars :: "stacked_prog_vars \<Rightarrow> symbolic_var \<Rightarrow> stacked_var_init \<Rightarrow> stacked_prog_vars" where
-"set_symbvar_in_prog_vars vars name val= 
+definition set_cur_symbvar_in_prog_vars :: "stacked_prog_vars \<Rightarrow> symbolic_var \<Rightarrow> stacked_var_init \<Rightarrow> stacked_prog_vars" where
+"set_cur_symbvar_in_prog_vars vars name val= 
   (case the (fmlookup vars name) of
     (stacked_prog_var.Var var) \<Rightarrow> (fmupd name (stacked_prog_var.Var val) vars)
   | (stacked_prog_var.InOutVar var) \<Rightarrow> (fmupd name (stacked_prog_var.InOutVar val) vars)
   | (stacked_prog_var.InVar var) \<Rightarrow> (fmupd name (stacked_prog_var.InVar val) vars)
   | (stacked_prog_var.OutVar var) \<Rightarrow> (fmupd name (stacked_prog_var.OutVar val) vars)
   | (stacked_prog_var.ExtVar var) \<Rightarrow> (fmupd name (stacked_prog_var.ExtVar val) vars))"
-declare set_symbvar_in_prog_vars_def [simp]
+declare set_cur_symbvar_in_prog_vars_def [simp]
 
-text "Setting symbolic var in current program in model state"
-definition set_cur_prog_symbvar :: "model_context \<Rightarrow> symbolic_var \<Rightarrow> stacked_var_init \<Rightarrow> model_context" where
-"set_cur_prog_symbvar st var_name val = 
-  (case st of (ST global_vars pg_map pg_name  f1 f2) \<Rightarrow>
-    (let (prog_vars,pc_map,pc_name) = the (fmlookup pg_map pg_name)
-     in (ST
-         global_vars 
-         (fmupd
-          pg_name
-          (set_symbvar_in_prog_vars prog_vars var_name val,
-           pc_map,
-           pc_name)
-          pg_map)
-         pg_name
-         f1
-         f2)))"
-declare set_cur_prog_symbvar_def [simp]
 
 text "Setting symbolic var in global vars"
-definition set_symbvar_in_global_vars :: "stacked_global_vars \<Rightarrow> symbolic_var \<Rightarrow> stacked_var_init \<Rightarrow> stacked_global_vars" where
-"set_symbvar_in_global_vars vars name val= 
+definition set_var_in_prog_vars_by_name :: "stacked_prog_vars \<Rightarrow> symbolic_var \<Rightarrow> stacked_var_init \<Rightarrow> stacked_prog_vars" where
+"set_var_in_prog_vars_by_name vars name val= 
   (case the (fmlookup vars name) of
-    (stacked_global_var.Var var) \<Rightarrow> (fmupd name (stacked_global_var.Var val) vars))"
-declare set_symbvar_in_global_vars_def [simp]
+    stacked_prog_var.Var var \<Rightarrow> (fmupd name (stacked_prog_var.Var val) vars)
+  | stacked_prog_var.ExtVar var \<Rightarrow> (fmupd name (stacked_prog_var.ExtVar val) vars)
+  | stacked_prog_var.InOutVar var \<Rightarrow> (fmupd name (stacked_prog_var.InOutVar val) vars)
+  | stacked_prog_var.InVar var \<Rightarrow> (fmupd name (stacked_prog_var.InVar val) vars)
+  | stacked_prog_var.OutVar var \<Rightarrow> (fmupd name (stacked_prog_var.OutVar val) vars))"
+declare set_var_in_prog_vars_by_name_def [simp]
+
+text "Setting program vars in current program context"
+definition set_cur_prog_vars :: "model_context \<Rightarrow> stacked_prog_vars \<Rightarrow> model_context" where
+"set_cur_prog_vars st vars = 
+(let (global_vars, pg_map, pg_name, f1, f2, v) = st; 
+     (pg_vars,pc_map,pc_name) = the (fmlookup pg_map pg_name) 
+in (global_vars, (fmupd pg_name (vars,pc_map,pc_name)  pg_map), pg_name, f1, f2, v))"
+declare set_cur_prog_vars_def [simp]
+
+(*(set_global_vars st (set_var_in_global_vars_by_name (get_global_vars st) var_name val))*)
+text "Setting symbolic var in current program in model state"
+definition set_cur_prog_var :: "model_context \<Rightarrow> symbolic_var \<Rightarrow> stacked_var_init \<Rightarrow> model_context" where
+"set_cur_prog_var st var_name val =
+  (set_cur_prog_vars st (set_var_in_prog_vars_by_name (get_cur_prog_vars st) var_name val))"
+declare set_cur_prog_var_def[simp]
+
+(*text "Setting symbolic var in current program in model state"
+definition set_cur_prog_var :: "model_context \<Rightarrow> symbolic_var \<Rightarrow> stacked_var_init \<Rightarrow> model_context" where
+"set_cur_prog_var st var_name val = 
+    (let (global_vars, pg_map, pg_name, f1, f2, value) = st;
+         (prog_vars,pc_map,pc_name) = the (fmlookup pg_map pg_name)
+     in (global_vars, 
+         (fmupd
+          pg_name
+          (set_cur_symbvar_in_prog_vars prog_vars var_name val,
+           pc_map,
+           pc_name)
+          pg_map),
+         pg_name,
+         f1,
+         f2,
+         value))"
+declare set_cur_prog_var_def [simp]*)
+
+text "Setting symbolic var in global vars"
+definition set_var_in_global_vars_by_name :: "stacked_global_vars \<Rightarrow> symbolic_var \<Rightarrow> stacked_var_init \<Rightarrow> stacked_global_vars" where
+"set_var_in_global_vars_by_name vars name val= 
+  (case (fmlookup vars name) of
+    Some (stacked_global_var.Var var) \<Rightarrow> (fmupd name (stacked_global_var.Var val) vars))"
+declare set_var_in_global_vars_by_name_def [simp]
 
 text "Setting global symbolic var in model state"
-definition set_global_symbvar :: "model_context \<Rightarrow> symbolic_var \<Rightarrow> stacked_var_init \<Rightarrow> model_context" where
-"set_global_symbvar st var_name val = 
-  (case st of (ST global_vars pg_map pg_name  funcs funblocks) \<Rightarrow>
-    (ST
-     (set_symbvar_in_global_vars global_vars var_name val) 
-     pg_map pg_name 
-     funcs
-     funblocks))"
-declare set_global_symbvar_def [simp]
+definition set_global_var :: "model_context \<Rightarrow> symbolic_var \<Rightarrow> stacked_var_init \<Rightarrow> model_context" where
+"set_global_var st var_name val = 
+  (set_global_vars st (set_var_in_global_vars_by_name (get_global_vars st) var_name val))"
+declare set_global_var_def [simp]
 
 text "Setting in model state new symbolic var value by name"
-definition set_symbvar :: "model_context \<Rightarrow> symbolic_var \<Rightarrow> basic_post_type => model_context" where
-"set_symbvar st var_name value =
+definition set_cur_symbvar :: "model_context \<Rightarrow> symbolic_var \<Rightarrow> ptype => model_context" where
+"set_cur_symbvar st var_name value =
   (let val = (stacked_var_init.Symbolic value None) in
-  (case (get_var_level_by_name_for_set st var_name) of
-    var_level.Global \<Rightarrow> (set_global_symbvar st var_name val)
-  | var_level.Program \<Rightarrow> (set_cur_prog_symbvar st var_name val)
-  | var_level.Process \<Rightarrow> (set_cur_proc_symbvar st var_name val)))"
-declare set_symbvar_def [simp]
+  (case (get_var_level_by_name st var_name) of
+    var_level.Global \<Rightarrow> (set_global_var st var_name val)
+  | var_level.Program \<Rightarrow> (set_cur_prog_var st var_name val)
+  | var_level.Process \<Rightarrow> (set_cur_proc_var st var_name val)))"
+declare set_cur_symbvar_def [simp]
 
-text "Setting new val to list in basic_post_type position"
-definition set_val_to_list_by_basic :: "'a list \<Rightarrow> basic_post_type \<Rightarrow> 'a \<Rightarrow> 'a list" where
+(*
+lemma
+  fixes st:: model_context and name :: symbolic_var and val :: ptype
+  assumes "var_exists st name"
+  shows"get_cur_symbvar_by_name (set_cur_symbvar st name val) name = val"
+  apply auto
+*)
+
+text "Setting new val to list in ptype position"
+definition set_val_to_list_by_basic :: "'a list \<Rightarrow> ptype \<Rightarrow> 'a \<Rightarrow> 'a list" where
 "set_val_to_list_by_basic l pos new_val = 
   (case pos of 
-    basic_post_type.Nat pos \<Rightarrow> (list_update l pos new_val) |
-    basic_post_type.Int pos \<Rightarrow> (list_update l (nat pos) new_val))"
+    ptype.Nat pos \<Rightarrow> (list_update l pos new_val) |
+    ptype.Int pos \<Rightarrow> (list_update l (nat pos) new_val))"
 declare set_val_to_list_by_basic_def [simp]
 
 text "Setting in model state new array variable single values by name and absolute position"
-definition set_arvar :: "model_context \<Rightarrow> symbolic_var \<Rightarrow> basic_post_type \<Rightarrow> basic_post_type \<Rightarrow>  model_context" where
+definition set_arvar :: "model_context \<Rightarrow> symbolic_var \<Rightarrow> ptype \<Rightarrow> ptype \<Rightarrow>  model_context" where
 "set_arvar st var_name pos value =
   (case (get_cur_var_init_by_name st var_name) of
     (stacked_var_init.Array (stacked_array_interval.Int val1 val2) values  opt) \<Rightarrow> 
       (let val = (stacked_var_init.Array 
                   (stacked_array_interval.Int val1 val2)
-                  (set_val_to_list_by_basic values (basic_post_type_sum (basic_post_type.Int val1) pos) value)
+                  (set_val_to_list_by_basic values (ptype_sum (ptype.Int val1) pos) value)
                   opt) in 
-  (case (get_var_level_by_name_for_set st var_name) of
-    var_level.Global \<Rightarrow> (set_global_symbvar st var_name val)
-  | var_level.Program \<Rightarrow> (set_cur_prog_symbvar st var_name val)
-  | var_level.Process \<Rightarrow> (set_cur_proc_symbvar st var_name val)))) "
+  (case (get_var_level_by_name st var_name) of
+    var_level.Global \<Rightarrow> (set_global_var st var_name val)
+  | var_level.Program \<Rightarrow> (set_cur_prog_var st var_name val)
+  | var_level.Process \<Rightarrow> (set_cur_proc_var st var_name val)))) "
 declare set_arvar_def [simp]
 
 text "Compare process status and estimated status"
-definition check_proc_status :: "model_context \<Rightarrow> process_name \<Rightarrow> proc_status \<Rightarrow> basic_post_type" where
+definition check_proc_status :: "model_context \<Rightarrow> process_name \<Rightarrow> proc_status \<Rightarrow> ptype" where
 "check_proc_status st name proc_stat = 
   (let (_,_,_,_, cur_proc_stat,_) = (get_procst_by_name st name) 
-    in (basic_post_type.Bool (proc_status_is cur_proc_stat proc_stat)))"
+    in (ptype.Bool (proc_status_is cur_proc_stat proc_stat)))"
 declare check_proc_status_def [simp]
 
 text "Setting current process name in current program"
 definition set_cur_proc_name :: "model_context \<Rightarrow> process_name \<Rightarrow> model_context" where
 "set_cur_proc_name st name = 
-  (case st of (ST g_list pg_map pg_name f1 f2) \<Rightarrow>
-      (let (var_list, p_map,p_name) = (get_cur_progst st)
-           
-        in (ST g_list 
-          (fmupd 
-              pg_name 
-              (var_list,p_map,name)
-              pg_map)
-            pg_name f1 f2)))"
+(let (global_vars, pg_map, pg_name, f1, f2, value) = st; 
+     (var_list, p_map,p_name) = (get_cur_progst st)
+  in (global_vars, 
+      (fmupd 
+        pg_name 
+        (var_list,p_map,name)
+        pg_map),
+       pg_name, f1, f2, value))"
 declare set_cur_proc_name_def [simp]
 
 text "Setting current program name"
 definition set_cur_prog_name :: "model_context \<Rightarrow> program_name \<Rightarrow> model_context" where
 "set_cur_prog_name st name =
-  (case st of
-    (ST g_list pg_map pg_name f1 f2) \<Rightarrow>
-      (ST g_list pg_map name f1 f2))"
+(let (global_vars, pg_map, pg_name, f1, f2, value) = st in (global_vars, pg_map, name, f1, f2, value))"
 declare set_cur_prog_name_def [simp]
 
 text "Resetting timer in current process in model state"
 definition reset_cur_timer :: "model_context \<Rightarrow> model_context" where
 "reset_cur_timer st = 
-  (case st of
-    (ST g_list pg_map pg_name fb_list f_list) \<Rightarrow>
-      (let (var_list, p_map,p_name) = (get_cur_progst st);
-           (process_vars, current_state, next_state, state_names, process_status, t) = (get_cur_procst_from_progst (var_list,p_map,p_name))
-        in (ST g_list 
-          (fmupd 
-              pg_name 
-              (var_list,(fmupd 
-                 p_name 
-                 (process_vars, current_state, next_state, state_names, process_status, time.Time 0 0 0 0 0)
-                 p_map),p_name)
-              pg_map) 
-            pg_name fb_list f_list)))"
+  (let (global_vars, pg_map, pg_name, f1, f2, value) = st;
+       (var_list, p_map,p_name) = (get_cur_progst st);
+       (process_vars, current_state, next_state, state_names, process_status, t) = (get_cur_procst_from_progst (var_list,p_map,p_name))
+   in (global_vars, 
+       (fmupd 
+         pg_name 
+         (var_list,(fmupd 
+          p_name 
+          (process_vars, current_state, next_state, state_names, process_status, time.Time 0 0 0 0 0)
+          p_map),p_name)
+       pg_map), 
+       pg_name, f1, f2, value))"
 declare reset_cur_timer_def [simp]
 
 text "Stopping process by name in model state"
 definition stop_process :: "model_context \<Rightarrow> process_name \<Rightarrow> model_context" where
 "stop_process st target_proc_name =
-    (case st of
-    (ST g_list pg_map pg_name fb_list f_list) \<Rightarrow>
-      (let (var_list, p_map,p_name) = (get_cur_progst st);
-           (process_vars, current_state, next_state, state_names, process_status, t) = (get_procst_from_progst_by_name (var_list,p_map,p_name) target_proc_name)
-        in (ST g_list 
+(let (global_vars, pg_map, pg_name, f1, f2, value) = st;
+     (var_list, p_map,p_name) = (get_cur_progst st);
+      (process_vars, current_state, next_state, state_names, process_status, t) = (get_procst_from_progst_by_name (var_list,p_map,p_name) target_proc_name)
+  in (global_vars, 
           (fmupd 
               pg_name 
               (var_list,(fmupd 
                  target_proc_name 
                  (process_vars, current_state, next_state, state_names, proc_status.Stop, t)
                  p_map),p_name)
-              pg_map) 
-            pg_name fb_list f_list)))"
+              pg_map), 
+            pg_name, f1, f2, value))"
 declare stop_process_def [simp]
 
 text "Stopping current process in model state"
 definition stop_cur_process :: "model_context  \<Rightarrow> model_context" where
 "stop_cur_process st =
-  (case st of
-    (ST g_list pg_map pg_name fb_list f_list) \<Rightarrow>
-      (let (var_list, p_map,p_name) = (get_cur_progst st);
-           (process_vars, current_state, next_state, state_names, process_status, t) = (get_procst_from_progst_by_name (var_list,p_map,p_name) p_name)
-        in (ST g_list 
+(let (global_vars, pg_map, pg_name, f1, f2, value) = st;
+     (var_list, p_map,p_name) = (get_cur_progst st);
+     (process_vars, current_state, next_state, state_names, process_status, t) = (get_procst_from_progst_by_name (var_list,p_map,p_name) p_name)
+  in (global_vars, 
           (fmupd 
               pg_name 
               (var_list,(fmupd 
                  p_name 
                  (process_vars, current_state, next_state, state_names, proc_status.Stop, t)
                  p_map),p_name)
-              pg_map) 
-            pg_name fb_list f_list)))"
+              pg_map), 
+            pg_name, f1, f2, value))"
 declare stop_cur_process_def [simp]
 
 text "Erroring process by name in model state"
 definition error_process :: "model_context \<Rightarrow> process_name \<Rightarrow> model_context" where
 "error_process st target_proc_name =
-   (case st of
-    (ST g_list pg_map pg_name fb_list f_list) \<Rightarrow>
-      (let (var_list, p_map,p_name) = (get_cur_progst st);
-           (process_vars, current_state, next_state, state_names, process_status, t) = (get_procst_from_progst_by_name (var_list,p_map,p_name) target_proc_name)
-        in (ST g_list 
+(let (global_vars, pg_map, pg_name, f1, f2, value) = st;
+     (var_list, p_map,p_name) = (get_cur_progst st);
+     (process_vars, current_state, next_state, state_names, process_status, t) = (get_procst_from_progst_by_name (var_list,p_map,p_name) target_proc_name)
+  in (global_vars, 
           (fmupd 
               pg_name 
               (var_list,(fmupd 
                  target_proc_name 
                  (process_vars, current_state, next_state, state_names, proc_status.Error, t)
                  p_map),p_name)
-              pg_map) 
-            pg_name fb_list f_list)))"
+              pg_map), 
+            pg_name, f1, f2, value))"
 declare error_process_def [simp]
 
 text "Erroring current process in model state"
 definition error_cur_process :: "model_context \<Rightarrow> model_context" where
 "error_cur_process st=
-   (case st of
-    (ST g_list pg_map pg_name fb_list f_list) \<Rightarrow>
-      (let (var_list, p_map,p_name) = (get_cur_progst st);
-           (process_vars, current_state, next_state, state_names, process_status, t) = (get_procst_from_progst_by_name (var_list,p_map,p_name) p_name)
-        in (ST g_list 
+(let (global_vars, pg_map, pg_name, f1, f2, value) = st;
+     (var_list, p_map,p_name) = (get_cur_progst st);
+     (process_vars, current_state, next_state, state_names, process_status, t) = (get_procst_from_progst_by_name (var_list,p_map,p_name) p_name)
+  in (global_vars, 
           (fmupd 
               pg_name 
               (var_list,(fmupd 
                  p_name 
                  (process_vars, current_state, next_state, state_names, proc_status.Error, t)
                  p_map),p_name)
-              pg_map) 
-            pg_name fb_list f_list)))"
+              pg_map), 
+            pg_name, f1, f2, value))"
 declare error_cur_process_def [simp]
 
 text "Resetting process by name in model state"
 definition reset_process :: "model_context \<Rightarrow> process_name \<Rightarrow> model_context" where
 "reset_process st target_proc_name =
- (case st of
-    (ST g_list pg_map pg_name fb_list f_list) \<Rightarrow>
-      (let (var_list, p_map,p_name) = (get_cur_progst st);
-           (process_vars, current_state, next_state, state_names, process_status, t) = (get_procst_from_progst_by_name (var_list,p_map,p_name) target_proc_name)
-        in (ST g_list 
+(let (global_vars, pg_map, pg_name, f1, f2, value) = st;
+     (var_list, p_map,p_name) = (get_cur_progst st);
+     (process_vars, current_state, next_state, state_names, process_status, t) = (get_procst_from_progst_by_name (var_list,p_map,p_name) target_proc_name)
+  in (global_vars, 
           (fmupd 
               pg_name 
               (var_list,(fmupd 
                  target_proc_name 
                  (process_vars, current_state, next_state, state_names, proc_status.Active, time.Time 0 0 0 0 0)
                  p_map),p_name)
-              pg_map) 
-            pg_name fb_list f_list)))"
+              pg_map), 
+            pg_name, f1, f2, value))"
 declare reset_process_def [simp]
 
 text "Resetting current process in model state"
 definition reset_cur_process :: "model_context \<Rightarrow> model_context" where
 "reset_cur_process st  =
- (case st of
-    (ST g_list pg_map pg_name fb_list f_list) \<Rightarrow>
-      (let (var_list, p_map,p_name) = (get_cur_progst st);
-           (process_vars, current_state, next_state, state_names, process_status, t) = (get_procst_from_progst_by_name (var_list,p_map,p_name) p_name)
-        in (ST g_list 
+(let (global_vars, pg_map, pg_name, f1, f2, value) = st;
+     (var_list, p_map,p_name) = (get_cur_progst st);
+     (process_vars, current_state, next_state, state_names, process_status, t) = (get_procst_from_progst_by_name (var_list,p_map,p_name) p_name)
+  in (global_vars,
           (fmupd 
               pg_name 
               (var_list,(fmupd 
                  p_name 
                  (process_vars, current_state, next_state, state_names, proc_status.Active, time.Time 0 0 0 0 0)
                  p_map),p_name)
-              pg_map) 
-            pg_name fb_list f_list)))"
+              pg_map), 
+            pg_name, f1, f2, value))"
 declare reset_cur_process_def [simp]
 
 definition inactive_cur_process :: "model_context \<Rightarrow> model_context" where
 "inactive_cur_process st =
-  (case st of
-    (ST g_list pg_map pg_name fb_list f_list) \<Rightarrow>
-      (let (var_list, p_map,p_name) = (get_cur_progst st);
-           (process_vars, current_state, next_state, state_names, process_status, t) = (get_procst_from_progst_by_name (var_list,p_map,p_name) p_name)
-        in (ST g_list 
+(let (global_vars, pg_map, pg_name, f1, f2, value) = st;
+     (var_list, p_map,p_name) = (get_cur_progst st);
+     (process_vars, current_state, next_state, state_names, process_status, t) = (get_procst_from_progst_by_name (var_list,p_map,p_name) p_name)
+  in (global_vars, 
           (fmupd 
               pg_name 
               (var_list,(fmupd 
                  p_name 
                  (process_vars, current_state, next_state, state_names, proc_status.Inactive, t)
                  p_map),p_name)
-              pg_map) 
-            pg_name fb_list f_list)))"
+              pg_map), 
+            pg_name, f1, f2, value))"
 declare inactive_cur_process_def [simp]
 
 definition inactive_process :: "model_context \<Rightarrow> process_name \<Rightarrow> model_context" where
 "inactive_process st target_proc_name =
-   (case st of
-    (ST g_list pg_map pg_name fb_list f_list) \<Rightarrow>
-      (let (var_list, p_map,p_name) = (get_cur_progst st);
-           (process_vars, current_state, next_state, state_names, process_status, t) = (get_procst_from_progst_by_name (var_list,p_map,p_name) target_proc_name)
-        in (ST g_list 
+(let (global_vars, pg_map, pg_name, f1, f2, value) = st;
+     (var_list, p_map,p_name) = (get_cur_progst st);
+     (process_vars, current_state, next_state, state_names, process_status, t) = (get_procst_from_progst_by_name (var_list,p_map,p_name) target_proc_name)
+  in (global_vars, 
           (fmupd 
               pg_name 
               (var_list,(fmupd 
                  target_proc_name 
                  (process_vars, current_state, next_state, state_names, proc_status.Inactive, t)
                  p_map),p_name)
-              pg_map) 
-            pg_name fb_list f_list)))"
+              pg_map), 
+            pg_name, f1, f2, value))"
 declare inactive_process_def [simp]
 
 text "Setting new state by name in current process in model state"
 definition set_state :: "model_context \<Rightarrow> state_name \<Rightarrow> model_context" where
 "set_state st st_name = 
-  (case st of
-    (ST g_list pg_map pg_name fb_list f_list) \<Rightarrow>
-      (let (var_list, p_map,p_name) = (get_cur_progst st);
-           (process_vars, current_state, next_state, state_names, process_status, t) = (get_procst_from_progst_by_name (var_list,p_map,p_name) p_name)
-        in (ST g_list 
+(let (global_vars, pg_map, pg_name, f1, f2, value) = st;
+     (var_list, p_map,p_name) = (get_cur_progst st);
+     (process_vars, current_state, next_state, state_names, process_status, t) = (get_procst_from_progst_by_name (var_list,p_map,p_name) p_name)
+  in (global_vars,
           (fmupd 
               pg_name 
               (var_list,(fmupd 
                  p_name 
                  (process_vars, current_state, st_name, state_names, process_status, t)
                  p_map),p_name)
-              pg_map) 
-            pg_name fb_list f_list)))"
+              pg_map), 
+            pg_name, f1, f2, value))"
 declare set_state_def [simp]
 
 text "Getting timeout of state"
 definition get_state_timeout :: "model_context \<Rightarrow> stacked_state \<Rightarrow> time" where
 "get_state_timeout st ss =
   (case ss of
-    (_,_,_, Some (timeout.Const t _)) => basic_to_time (const_to_basic t)
-  | (_,_,_, Some (timeout.SymbolicVar var_name _)) => basic_to_time (get_cur_symbvar_by_name st var_name))"
+    (_,_, Some (timeout.Const t _)) => basic_to_time (const_to_basic t)
+  | (_,_, Some (timeout.SymbolicVar var_name _)) => basic_to_time (get_cur_symbvar_by_name st var_name))"
 declare get_state_timeout_def [simp]
 
 text "Getting time of current process"
 definition get_cur_time :: "model_context \<Rightarrow> time" where
 "get_cur_time st = 
- (case st of (ST global_var_decl_list pg_map p_name function_block_decl_list function_decl_list) \<Rightarrow>
-    (let (var_list,proc_map, proc_name) = (case (fmlookup pg_map p_name) of Some(p_state) \<Rightarrow> p_state);
+(let (global_vars, pg_map, pg_name, f1, f2, value) = st;
+     (var_list,proc_map, proc_name) = (case (fmlookup pg_map pg_name) of Some(p_state) \<Rightarrow> p_state);
         (proc_vars,st_name,next_state,state_names, proc_stat, cur_time) = (case (fmlookup proc_map proc_name) of Some(proc_state) \<Rightarrow> proc_state)
-    in cur_time)) "
+    in cur_time) "
 declare get_cur_time_def [simp]
 
 text "Getting time of process by name"
 definition get_process_time_by_name :: "model_context \<Rightarrow> process_name \<Rightarrow> time" where
 "get_process_time_by_name st proc_name= 
- (case st of (ST global_var_decl_list pg_map pg_name  function_block_decl_list function_decl_list) \<Rightarrow>
-    (let (var_list,proc_map, _) = (case (fmlookup pg_map pg_name) of Some(p_state) \<Rightarrow> p_state);
+(let (global_vars, pg_map, pg_name, f1, f2, value) = st;
+     (var_list,proc_map, _) = (case (fmlookup pg_map pg_name) of Some(p_state) \<Rightarrow> p_state);
         ((proc_var_list),st_name,next_state,state_names, proc_stat, cur_time) = (case (fmlookup proc_map proc_name) of Some(proc_state) \<Rightarrow> proc_state)
-  in cur_time)) "
+  in cur_time) "
 declare get_process_time_by_name_def [simp]
 
 text "Getting name of next state"
@@ -522,13 +579,12 @@ declare get_next_state_name.simps [simp]
 text "Setting next state name in next state"
 definition set_next_state_next :: "model_context \<Rightarrow> model_context" where
 "set_next_state_next st = 
- (case st of (ST global_var_decl_list pg_map pg_name function_block_decl_list function_decl_list) \<Rightarrow>
-    (let (var_list,proc_map, proc_name) = (case (fmlookup pg_map pg_name) of Some(p_state) \<Rightarrow> p_state);
+(let (global_vars, pg_map, pg_name, f1, f2, value) = st;
+     (var_list,proc_map, proc_name) = (case (fmlookup pg_map pg_name) of Some(p_state) \<Rightarrow> p_state);
         ((proc_var_list),st_name,next_state,state_names, proc_stat, cur_time) = (case (fmlookup proc_map proc_name) of 
                                     Some(proc_state) \<Rightarrow> proc_state);
     next_state_name = get_next_state_name state_names st_name
-  in (ST 
-        global_var_decl_list 
+  in (global_vars, 
         (fmupd 
             pg_name
             (var_list,(fmupd 
@@ -536,21 +592,18 @@ definition set_next_state_next :: "model_context \<Rightarrow> model_context" wh
                  ((proc_var_list), st_name,next_state_name,state_names, proc_stat, cur_time)
                  proc_map), 
               proc_name) 
-            pg_map)
-          pg_name 
-        function_block_decl_list 
-        function_decl_list))) " 
+            pg_map),
+          pg_name, f1, f2, value)) " 
 declare set_next_state_next_def [simp]
 
 text "Setting current state into next state"
 definition set_into_next_state :: "model_context \<Rightarrow> model_context" where
 "set_into_next_state st = 
- (case st of (ST global_var_decl_list pg_map pg_name  function_block_decl_list function_decl_list) \<Rightarrow>
-    (let (var_list,proc_map, proc_name) = (case (fmlookup pg_map pg_name) of Some(p_state) \<Rightarrow> p_state);
+(let (global_vars, pg_map, pg_name, f1, f2, value) = st;
+     (var_list,proc_map, proc_name) = (case (fmlookup pg_map pg_name) of Some(p_state) \<Rightarrow> p_state);
         ((proc_var_list),st_name,next_state,state_names, proc_stat, cur_time) = (case (fmlookup proc_map proc_name) of 
                                     Some(proc_state) \<Rightarrow> proc_state) 
-  in (ST 
-        global_var_decl_list 
+  in (global_vars, 
         (fmupd 
             pg_name
             (var_list,(fmupd 
@@ -558,22 +611,20 @@ definition set_into_next_state :: "model_context \<Rightarrow> model_context" wh
                  (proc_var_list, next_state,next_state,state_names, proc_stat, (if (st_name = next_state) then cur_time else (time.Time 0 0 0 0 0)))
                  proc_map), 
               proc_name) 
-            pg_map)
-          pg_name 
-        function_block_decl_list 
-        function_decl_list))) " 
+            pg_map),
+          pg_name, f1, f2, value)) " 
 declare set_into_next_state_def [simp]
 
 text "Extract timeout stmt if cur process time more than timeout "
 definition extr_timeout_stmt :: "model_context \<Rightarrow> timeout \<Rightarrow> (stmt option)" where
 "extr_timeout_stmt st timeo = 
-  (case st of (ST global_var_decl_list pg_map pg_name function_block_decl_list function_decl_list) \<Rightarrow>
-    (let (var_list,proc_map, proc_name) = (case (fmlookup pg_map pg_name) of Some(p_state) \<Rightarrow> p_state);
+(let (global_vars, pg_map, pg_name, f1, f2, value) = st;
+     (var_list,proc_map, proc_name) = (case (fmlookup pg_map pg_name) of Some(p_state) \<Rightarrow> p_state);
         ((proc_var_list),st_name,next_state,state_names, proc_stat, cur_time) = (case (fmlookup proc_map proc_name) of 
                                     Some(proc_state) \<Rightarrow> proc_state) 
   in (case timeo of
        (timeout.Const c stm) \<Rightarrow>  (if (time_less (basic_to_time (const_to_basic c)) cur_time) then (Some stm) else None)
-     | (timeout.SymbolicVar sv stm) \<Rightarrow> (if (time_less (basic_to_time (get_cur_symbvar_by_name st sv)) cur_time) then (Some stm) else None))))"
+     | (timeout.SymbolicVar sv stm) \<Rightarrow> (if (time_less (basic_to_time (get_cur_symbvar_by_name st sv)) cur_time) then (Some stm) else None)))"
 declare extr_timeout_stmt_def [simp]
 
 text "Gather out and inout vars from process vars"
@@ -627,17 +678,17 @@ declare update_processes_in_vars_def [simp]
 text "Distribution of process out vars values"
 definition process_vars_distribution :: "model_context \<Rightarrow> model_context" where
 "process_vars_distribution st = 
-  (case st of (ST global_var_decl_list pg_map pg_name f1 f2) \<Rightarrow>
-    (let (var_list,proc_map, proc_name) = (case (fmlookup pg_map pg_name) of Some(p_state) \<Rightarrow> p_state);
+(let (global_vars, pg_map, pg_name, f1, f2, value) = st;
+     (var_list,proc_map, proc_name) = (case (fmlookup pg_map pg_name) of Some(p_state) \<Rightarrow> p_state);
         put_vars = gather_processes_out_vars proc_map 
-  in (ST global_var_decl_list 
+  in (global_vars,
       (fmupd
         pg_name
         (var_list,
           update_processes_in_vars proc_map put_vars,
           proc_name)
-        pg_map)
-      pg_name f1 f2)))"
+        pg_map),
+      pg_name, f1, f2, value))"
 declare process_vars_distribution_def [simp]
 
 text "gather Out and InOut vars from program vars"
@@ -691,20 +742,19 @@ declare update_programs_in_vars_def [simp]
 text "Distribution of program out vars values"
 definition prog_vars_distribution :: "model_context \<Rightarrow> model_context" where
 "prog_vars_distribution st = 
-  (case st of (ST global_var_decl_list ps_map p_name f1 f2) \<Rightarrow>
-    (let put_vars = gather_programs_out_vars ps_map 
-  in (ST global_var_decl_list
-      (update_programs_in_vars ps_map put_vars)
-      p_name f1 f2)))"
+(let (global_vars, pg_map, pg_name, f1, f2, value) = st;
+     put_vars = gather_programs_out_vars pg_map 
+  in (global_vars,
+      (update_programs_in_vars pg_map put_vars),
+      pg_name, f1, f2, value))"
 declare prog_vars_distribution_def [simp]
 
 text "Incrementing active processes time by time step"
 definition add_time_to_active_processes :: "model_context \<Rightarrow> time \<Rightarrow> model_context" where
 "add_time_to_active_processes st t = 
-  (case st of (ST global_var_decl_list pg_map pg_name function_block_decl_list function_decl_list) \<Rightarrow>
-    (let (var_list,proc_map, proc_name) = (case (fmlookup pg_map pg_name) of Some(p_state) \<Rightarrow> p_state)
-  in (ST 
-        global_var_decl_list 
+(let (global_vars, pg_map, pg_name, f1, f2, value) = st;
+     (var_list,proc_map, proc_name) = (case (fmlookup pg_map pg_name) of Some(p_state) \<Rightarrow> p_state)
+  in (global_vars, 
         (fmmap
             (\<lambda>(vars,pc_map,pc_name). 
               (vars,
@@ -713,28 +763,27 @@ definition add_time_to_active_processes :: "model_context \<Rightarrow> time \<R
                 (v1,v2,v3,v4,stat, (if (proc_status_is stat proc_status.Active) then (time_sum t1 t) else t1)))
               pc_map,
               pc_name))
-            pg_map)
-          pg_name
-        function_block_decl_list 
-        function_decl_list)))"
+            pg_map),
+          pg_name, f1, f2, value))"
 declare add_time_to_active_processes_def [simp]
 
 text "Checking is process active by name"
 definition is_process_active :: "model_context \<Rightarrow> process_name \<Rightarrow> bool" where
 "is_process_active st name = 
-  (case st of (ST global_var_decl_list pg_map pg_name function_block_decl_list function_decl_list) \<Rightarrow>
-    (let (var_list,proc_map, proc_name) = (case (fmlookup pg_map pg_name) of Some(p_state) \<Rightarrow> p_state);
+(let (global_vars, pg_map, pg_name, f1, f2, value) = st;
+     (var_list,proc_map, proc_name) = (case (fmlookup pg_map pg_name) of Some(p_state) \<Rightarrow> p_state);
          (_,_,_,_,status,_) = (case (fmlookup proc_map name) of Some(proc_state) \<Rightarrow> proc_state)
-    in (proc_status_is status proc_status.Active)))"
+    in (proc_status_is status proc_status.Active))"
 declare is_process_active_def [simp]
 
 text "Getting function body by name"
 definition get_func_by_name :: "model_context \<Rightarrow> func_name \<Rightarrow> stacked_func" where
 "get_func_by_name st name = 
-  (case st of (ST _ _ _ _ f_map) \<Rightarrow> the (fmlookup f_map name))"
+(let (global_vars, pg_map, pg_name, f1, f2, value) = st in 
+  the (fmlookup f2 name))"
 declare get_func_by_name_def [simp] 
 
 declare fmupd_reorder_neq [simp]
-(*declare fmran_def [simp]
-declare ffold_def [simp]*)
+declare fmran_def [simp]
+declare ffold_def [simp]
 end
