tests/poST_HandDryer.thy
@@ -7,16 +7,17 @@ definition HandDryer :: "model" where
 "HandDryer = 
   (None,[],
   [(''HandDryer'',
-    [(prog_var.InVar ( [(''hands'',var_init_decl.Symbolic (basic_post_type.Bool False) None)])),
-     (prog_var.OutVar ( [(''control'',var_init_decl.Symbolic (basic_post_type.Bool False) None)]))],
+    [(prog_var.InVar ( [(''hands'',var_init_decl.Symbolic (ptype.Bool False) None)])),
+     (prog_var.OutVar ( [(''control'',var_init_decl.Symbolic (ptype.Bool False) None)]))],
     [(''Init'',
      [],
      [(''Wait'',
        False,
        [(statement.SelectSt 
-          (select_statement.IfSt [(expr.SymbolicVar ''hands'',
-                                  [statement.AssignSt (common_var.Symbolic ''control'') (expr.Const (const.Bool True)),
-                                   statement.SetStateSt None])] None))],
+          (select_statement.IfSt 
+            [(expr.SymbolicVar ''hands'',
+              [statement.AssignSt (common_var.Symbolic ''control'') (expr.Const (const.Bool True)),
+               statement.SetStateSt None])] None))],
        None),
        (''Work'',
         False,
@@ -49,11 +50,11 @@ definition model_time :: "time" where
 declare model_time_def [simp]
 
 definition set_hands :: "model_context \<Rightarrow> model_context" where
-"set_hands st = set_symbvar st ''hands'' (basic_post_type.Bool True)"
+"set_hands st = set_cur_symbvar st ''hands'' (ptype.Bool True)"
 declare set_hands_def [simp]
 
 definition remove_hands :: "model_context \<Rightarrow> model_context" where
-"remove_hands st = set_symbvar st ''hands'' (basic_post_type.Bool False)"
+"remove_hands st = set_cur_symbvar st ''hands'' (ptype.Bool False)"
 declare remove_hands_def [simp]
 
 
@@ -71,7 +72,7 @@ schematic_goal "model_time:stacked_HandDaryer_model\<turnstile>stacked_HandDryer
      apply (rule StateStep)
        apply (rule IfF)
         apply (auto)
-         apply (rule Var)
+         apply (rule Symbolic)
          apply (auto)
        apply (rule Blank)
     apply (rule ProcNil)
@@ -92,7 +93,7 @@ schematic_goal "model_time:(set_hands stacked_HandDaryer_model)\<turnstile>stack
      apply (rule StateStep)
        apply (rule IfT)
         apply (auto)
-         apply (rule Var)
+         apply (rule Symbolic)
         apply (auto)
       apply (rule Comb)
        apply (rule AssignS)
@@ -105,7 +106,7 @@ schematic_goal "model_time:(set_hands stacked_HandDaryer_model)\<turnstile>stack
   done
 
 definition set_control :: "model_context \<Rightarrow> model_context" where
-"set_control st = set_symbvar st ''control'' (basic_post_type.Bool True)"
+"set_control st = set_cur_symbvar st ''control'' (ptype.Bool True)"
 declare set_control_def [simp]
 
 schematic_goal "model_time:(set_control stacked_HandDaryer_model)\<turnstile>stacked_HandDryer\<mapsto>?st"
@@ -117,7 +118,7 @@ schematic_goal "model_time:(set_control stacked_HandDaryer_model)\<turnstile>sta
     apply (rule ProcStep) apply (auto)
     apply (rule StateStep)
       apply (rule IfF) apply (auto)
-        apply (rule Var) apply (auto)
+        apply (rule Symbolic) apply (auto)
       apply (rule Blank)
    apply (rule ProcNil)
   apply (rule ProgNil)
@@ -130,7 +131,7 @@ declare set_overtime_def [simp]
 definition set_work_state :: "model_context \<Rightarrow> model_context" where
 "set_work_state st = set_into_next_state (set_state st ''Work'')"
 declare set_work_state_def [simp]
-
+(*
 schematic_goal "model_time:(set_work_state (set_overtime (set_control stacked_HandDaryer_model)))\<turnstile>stacked_HandDryer\<mapsto>?st"
   apply (auto)
   apply (rule ModelStep) apply (auto)
@@ -140,7 +141,7 @@ schematic_goal "model_time:(set_work_state (set_overtime (set_control stacked_Ha
      apply (rule ProcStep) apply (auto)
        apply (rule StateStep)
          apply (rule IfF) apply (auto)
-           apply (rule Var) apply (auto)
+           apply (rule Symbolic) apply (auto)
      apply (rule Blank) apply (auto)
     apply (rule Comb)
      apply (rule AssignS) apply (auto)
@@ -149,32 +150,27 @@ schematic_goal "model_time:(set_work_state (set_overtime (set_control stacked_Ha
    apply (rule ProcNil)
   apply (rule ProgNil)
   done
+*) 
 
-lemma 
-"st\<turnstile>stmt.AssignSt (common_var.Symbolic ''hands'') (expr.Const (const.Nat 1)) \<longrightarrow> st1 \<Longrightarrow>
- basic_post_type_eq (get_cur_symbvar_by_name st1 ''hands'') (basic_post_type.Nat 1)"
-  apply (induction st1 arbitrary:st)
-  apply auto
-  apply (rule )
 
-(*
-text "If the dryer is on, then it turns off after no hands are present for 1 second."
+
+text "If the dryer is on, then it turns off after no hands are present for 2 second."
 lemma
-  "model_time:stacked_HandDaryer_model\<turnstile>stacked_HandDryer\<mapsto>st \<Longrightarrow> 
-  time_more (get_cur_time stacked_HandDaryer_model) (time 0 0 0 1 0) \<Longrightarrow>
-  \<not>(basic_post_type_to_bool (get_cur_symbvar_by_name stacked_HandDaryer_model ''hands'')) \<Longrightarrow>
-  \<not>(basic_post_type_to_bool (get_cur_symbvar_by_name st ''control''))"
+  assumes "time_step:st\<turnstile>stacked_HandDryer\<mapsto>st1" 
+  and     "time_more (get_cur_time st) (time.Time 0 0 0 2 0)" 
+  and     "\<not>(ptype_to_bool (get_cur_symbvar_by_name st ''hands''))" 
+  shows   "\<not>(ptype_to_bool (get_cur_symbvar_by_name st1 ''control''))"
 proof 
 qed
-*)
+
 
 (*
 text "If the dryer was not turned on and hands appeared, it will turn on ASAP."
 lemma
   "model_time:stacked_HandDaryer_model\<turnstile>stacked_HandDryer\<mapsto>st \<Longrightarrow> 
-  \<not>(basic_post_type_to_bool (get_cur_symbvar_by_name stacked_HandDaryer_model ''control'')) 
-  (basic_post_type_to_bool (get_cur_symbvar_by_name stacked_HandDaryer_model ''hands'')) \<Longrightarrow>
-  (basic_post_type_to_bool (get_cur_symbvar_by_name st ''control''))"
+  \<not>(ptype_to_bool (get_cur_symbvar_by_name stacked_HandDaryer_model ''control'')) 
+  (ptype_to_bool (get_cur_symbvar_by_name stacked_HandDaryer_model ''hands'')) \<Longrightarrow>
+  (ptype_to_bool (get_cur_symbvar_by_name st ''control''))"
 proof sorry
 qed
 *)
@@ -183,9 +179,9 @@ qed
 text "If the hands are present and the dryer is on, it will not turn off."
 lemma
   "model_time:stacked_HandDaryer_model\<turnstile>stacked_HandDryer\<mapsto>st \<Longrightarrow> 
-  (basic_post_type_to_bool (get_cur_symbvar_by_name stacked_HandDaryer_model ''hands'')) \<Longrightarrow>
-  (basic_post_type_to_bool (get_cur_symbvar_by_name stacked_HandDaryer_model ''control'')) \<Longrightarrow>
-  (basic_post_type_to_bool (get_cur_symbvar_by_name st ''control''))"
+  (ptype_to_bool (get_cur_symbvar_by_name stacked_HandDaryer_model ''hands'')) \<Longrightarrow>
+  (ptype_to_bool (get_cur_symbvar_by_name stacked_HandDaryer_model ''control'')) \<Longrightarrow>
+  (ptype_to_bool (get_cur_symbvar_by_name st ''control''))"
 proof sorry
 qed
 *)
@@ -194,9 +190,9 @@ qed
 text "If there is no hands and the dryer is not turned on, the dryer will not turn on until the hands appear."
 lemma
   "model_time:stacked_HandDaryer_model\<turnstile>stacked_HandDryer\<mapsto>st \<Longrightarrow> 
-  \<not>(basic_post_type_to_bool (get_cur_symbvar_by_name stacked_HandDaryer_model ''hands'')) \<Longrightarrow>
-  \<not>(basic_post_type_to_bool (get_cur_symbvar_by_name stacked_HandDaryer_model ''control'')) \<Longrightarrow>
-  \<not>(basic_post_type_to_bool (get_cur_symbvar_by_name st ''control''))"
+  \<not>(ptype_to_bool (get_cur_symbvar_by_name stacked_HandDaryer_model ''hands'')) \<Longrightarrow>
+  \<not>(ptype_to_bool (get_cur_symbvar_by_name stacked_HandDaryer_model ''control'')) \<Longrightarrow>
+  \<not>(ptype_to_bool (get_cur_symbvar_by_name st ''control''))"
 proof sorry
 qed
 *)
