poSTVM/poSTVM_alt_inductive.thy
@@ -53,52 +53,63 @@ definition update_process_status :: "model_context \<Rightarrow> process_stateme
 declare update_process_status_def [simp]
 
 inductive 
-  eval :: "[model_context, expr, model_context * basic_post_type] \<Rightarrow> bool" ("_ \<turnstile> _ \<rightarrow> _") and
+  eval :: "[model_context, expr, model_context] \<Rightarrow> bool" ("_ \<turnstile> _ \<rightarrow> _") and
   exec :: "[model_context,stmt,model_context] \<Rightarrow> bool" ("_ \<turnstile> _ \<longrightarrow> _") and
-  exec_func :: "[model_context,func_name,func_params,model_context*basic_post_type] \<Rightarrow> bool" ("_\<turnstile>_,_\<longrightarrow> _") and
+  exec_func :: "[model_context,func_name,func_params,model_context] \<Rightarrow> bool" ("_\<turnstile>_,_\<longrightarrow> _") and
   assign_param :: "[model_context,assign_type,param_assign list,model_context,model_context] \<Rightarrow> bool"
   where
-    BinOp : "\<lbrakk>st\<turnstile>exp1\<rightarrow>(st1,val1);
-              st1\<turnstile>exp2\<rightarrow>(st2,val2);
+    BinOp : "\<lbrakk>st\<turnstile>exp1\<rightarrow>st1;
+              val1 = get_value st1;
+              st1\<turnstile>exp2\<rightarrow>st2;
+              val2 = get_value st2;
               val = binary_op_exec bin_op val1 val2 \<rbrakk> \<Longrightarrow>
-             st\<turnstile>expr.Binary bin_op exp1 exp2\<rightarrow>(st2,val)"
-  | UnOp : "\<lbrakk>st\<turnstile>pexp\<rightarrow>(st1,val1);
-                val = (unary_op_exec un_op val1)\<rbrakk> \<Longrightarrow>
-               st\<turnstile> expr.Unary un_op pexp\<rightarrow>(st1,val)"
-  | Const : "\<lbrakk>val = const_to_basic c\<rbrakk>\<Longrightarrow>
-            st\<turnstile>expr.Const c\<rightarrow>(st,val)"
-  | Var :  "\<lbrakk>val = get_cur_symbvar_by_name st var_name\<rbrakk>\<Longrightarrow>
-           st\<turnstile>expr.SymbolicVar var_name\<rightarrow>(st,val)"
-  | ArrayVar : "\<lbrakk>st\<turnstile>exp\<rightarrow>(_,pos);
-                 val = get_cur_arvar_by_name_by_pos st var_name pos\<rbrakk>\<Longrightarrow>
-               st\<turnstile>expr.ArrayVar var_name exp\<rightarrow>(st,val)"
+              st\<turnstile>expr.Binary bin_op exp1 exp2\<rightarrow>(set_value st2 val)"
+  | UnOp : "\<lbrakk>st\<turnstile>pexp\<rightarrow>st1;
+             val1 = get_value st1;
+             val = (unary_op_exec un_op val1)\<rbrakk> \<Longrightarrow>
+             st\<turnstile> expr.Unary un_op pexp\<rightarrow>(set_value st1 val)"
+  | Const : "\<lbrakk>st1 = (set_value st (const_to_basic c))\<rbrakk>\<Longrightarrow>
+              st\<turnstile>expr.Const c\<rightarrow>st1"
+  | Symbolic :  "\<lbrakk>val = get_cur_symbvar_by_name st var_name;
+                  st1 = (set_value st val)\<rbrakk>\<Longrightarrow>
+                  st\<turnstile>expr.SymbolicVar var_name\<rightarrow>st1"
+  | Array : "\<lbrakk>st\<turnstile>exp\<rightarrow>st1;
+              pos = get_value st1;
+              val = get_cur_arvar_by_name_by_pos st1 var_name pos\<rbrakk>\<Longrightarrow>
+              st\<turnstile>expr.ArrayVar var_name exp\<rightarrow>(set_value st1 val)"
   | PSE : "\<lbrakk>val = check_proc_status st p_name p_status\<rbrakk>\<Longrightarrow>
-          st\<turnstile>expr.ProcStatEpxr p_name p_status\<rightarrow>(st,val)"
- |FuncCall : "\<lbrakk>st\<turnstile>name,as_list\<longrightarrow>(st1,val)\<rbrakk> \<Longrightarrow> st\<turnstile>expr.FunctionCall name as_list \<rightarrow> (st1,val)"
+            st\<turnstile>expr.ProcStatEpxr p_name p_status\<rightarrow>(set_value st val)"
+  | FuncCall : "\<lbrakk>st\<turnstile>name,as_list\<longrightarrow>st1\<rbrakk> \<Longrightarrow> 
+                 st\<turnstile>expr.FunctionCall name as_list \<rightarrow> st1"
 
   | Blank : "st\<turnstile>stmt.Blank\<longrightarrow>st"
   | Comb : "\<lbrakk>st\<turnstile>s1\<longrightarrow>st1;
              st1\<turnstile>s2\<longrightarrow>st2\<rbrakk>\<Longrightarrow>
            st\<turnstile>stmt.Comb s1 s2 \<longrightarrow>st2"
-  | IfT : "\<lbrakk>st\<turnstile>exp\<rightarrow>(st_res,val);
-            (basic_post_type_to_bool val);
-            st\<turnstile>s1\<longrightarrow>st1\<rbrakk>\<Longrightarrow>
-         st\<turnstile>stmt.IfSt exp s1 s2\<longrightarrow>st1"
-  | IfF : "\<lbrakk>st\<turnstile>exp\<rightarrow>(st_res,val);
-           \<not>(basic_post_type_to_bool val);
-           st\<turnstile>s2\<longrightarrow>st1\<rbrakk> \<Longrightarrow> st\<turnstile>stmt.IfSt exp s1 s2\<longrightarrow>st1"
-  | LoopF : "\<lbrakk>st\<turnstile>exp\<rightarrow>(st_sub,val); \<not>(basic_post_type_to_bool val)\<rbrakk>\<Longrightarrow>
-            st\<turnstile>stmt.WhileSt exp s\<longrightarrow>st"
-  | LoopT : "\<lbrakk>st\<turnstile>exp\<rightarrow>(st_sub,val); (basic_post_type_to_bool val);
-              st\<turnstile>s\<longrightarrow>st1;st1\<turnstile>stmt.WhileSt exp s\<longrightarrow>st2\<rbrakk>\<Longrightarrow>
-              st\<turnstile>stmt.WhileSt exp s\<longrightarrow>st2"
-  | AssignS : "\<lbrakk>st\<turnstile>exp\<rightarrow>(st1,val);
-                st2 = (set_symbvar st1 var_name val)\<rbrakk>\<Longrightarrow>
-              st\<turnstile>stmt.AssignSt (common_var.Symbolic var_name) exp\<longrightarrow>st2"
-  | AssignA : "\<lbrakk>st\<turnstile>exp\<rightarrow>(st1,val1);
-                st1\<turnstile>pos\<rightarrow>(st1,val2);
-                st2 = (set_arvar st1 var_name val2 val1)\<rbrakk>\<Longrightarrow>
-              st\<turnstile>stmt.AssignSt (common_var.Array var_name pos) exp\<longrightarrow>st2"
+  | IfT : "\<lbrakk>st\<turnstile>exp\<rightarrow>st1;
+            (ptype_to_bool (get_value st1));
+            st1\<turnstile>s1\<longrightarrow>st2\<rbrakk>\<Longrightarrow>
+         st\<turnstile>stmt.IfSt exp s1 s2\<longrightarrow>st2"
+  | IfF : "\<lbrakk>st\<turnstile>exp\<rightarrow>st1;
+           \<not>(ptype_to_bool (get_value st1));
+           st1\<turnstile>s2\<longrightarrow>st2\<rbrakk> \<Longrightarrow> st\<turnstile>stmt.IfSt exp s1 s2\<longrightarrow>st2"
+  | LoopF : "\<lbrakk>st\<turnstile>exp\<rightarrow>st1; 
+              \<not>(ptype_to_bool (get_value st1))\<rbrakk>\<Longrightarrow>
+              st\<turnstile>stmt.WhileSt exp s\<longrightarrow>st1"
+  | LoopT : "\<lbrakk>st\<turnstile>exp\<rightarrow>st1; 
+              (ptype_to_bool (get_value st1));
+              st1\<turnstile>s\<longrightarrow>st2;
+              st2\<turnstile>stmt.WhileSt exp s\<longrightarrow>st3\<rbrakk>\<Longrightarrow>
+              st\<turnstile>stmt.WhileSt exp s\<longrightarrow>st3"
+  | AssignS : "\<lbrakk>st\<turnstile>exp\<rightarrow>st1;
+                st2 = (set_cur_symbvar st1 var_name (get_value st1))\<rbrakk>\<Longrightarrow>
+                st\<turnstile>stmt.AssignSt (common_var.Symbolic var_name) exp\<longrightarrow>st2"
+  | AssignA : "\<lbrakk>st\<turnstile>exp\<rightarrow>st1;
+                val1 = get_value st1;
+                st1\<turnstile>pos\<rightarrow>st2;
+                val2 = get_value st2;
+                st3 = (set_arvar st2 var_name val2 val1)\<rbrakk>\<Longrightarrow>
+              st\<turnstile>stmt.AssignSt (common_var.Array var_name pos) exp\<longrightarrow>st3"
   | Return : "st\<turnstile>stmt.Return\<longrightarrow>st"
   | Exit : "st\<turnstile>stmt.Exit\<longrightarrow>st"
   | ProcessStart : "\<lbrakk>st1 = (case stm_name_option of None \<Rightarrow> reset_cur_process st | Some name \<Rightarrow> reset_process st name)\<rbrakk> \<Longrightarrow> 
@@ -119,49 +130,68 @@ inductive
                   as_proxy_state\<turnstile>stmts\<longrightarrow>st1;
                   assign_param st1 assign_type.Conseq params st new_st;
                   res = (get_cur_symbvar_by_name st1 f_name)\<rbrakk>\<Longrightarrow>
-                st\<turnstile>name,params\<longrightarrow>(new_st,res)"
+                st\<turnstile>name,params\<longrightarrow>(set_value new_st res)"
   | AssignPNill : "assign_param base_st type [] st st"
-  | AssignPConsCol : "\<lbrakk>base_st \<turnstile> exp \<rightarrow> (st,val);
+  | AssignPConsCol : "\<lbrakk>base_st \<turnstile> exp \<rightarrow> st;
+                       val = get_value st;
                        (if as_type = assign_type.ColonEq 
-                        then (assign_param base_st assign_type.ColonEq other (set_symbvar st name val) new_st)
+                        then (assign_param base_st assign_type.ColonEq other (set_cur_symbvar st name val) new_st)
                         else (assign_param base_st assign_type.ColonEq other st new_st))\<rbrakk> \<Longrightarrow> 
                       assign_param base_st assign_type.ColonEq ((param_assign.SymbolicVar name as_type exp)#other) st new_st"
-  | AssignPConsCon : "\<lbrakk>base_st \<turnstile> exp \<rightarrow> (st,val);
+  | AssignPConsCon : "\<lbrakk>base_st \<turnstile> exp \<rightarrow> st;
+                       val = get_value st;
                        (if as_type = assign_type.Conseq 
                         then (assign_param base_st assign_type.Conseq other st new_st) 
-                        else (assign_param base_st assign_type.Conseq other (set_symbvar st name val) new_st))  \<rbrakk> \<Longrightarrow> 
+                        else (assign_param base_st assign_type.Conseq other (set_cur_symbvar st name val) new_st))  \<rbrakk> \<Longrightarrow> 
                       assign_param base_st assign_type.Conseq ((param_assign.SymbolicVar name as_type exp)#other) st new_st"
 
 print_theorems 
 
 text "eval code_pred_intro lemmas"
 lemma [code_pred_intro]: 
-"\<lbrakk>st\<turnstile>exp1\<rightarrow>(st1,val1);
-              st1\<turnstile>exp2\<rightarrow>(st2,val2);
+"\<lbrakk>st\<turnstile>exp1\<rightarrow>st1;
+              val1 = get_value st1;
+              st1\<turnstile>exp2\<rightarrow>st2;
+              val2 = get_value st2;
               val = binary_op_exec bin_op val1 val2 \<rbrakk> \<Longrightarrow>
-             st\<turnstile>expr.Binary bin_op exp1 exp2\<rightarrow>(st2,val)"
-"\<lbrakk>st\<turnstile>pexp\<rightarrow>(st1,val1);
-                val = (unary_op_exec un_op val1)\<rbrakk> \<Longrightarrow>
-               st\<turnstile> expr.Unary un_op pexp\<rightarrow>(st1,val)"
+              st\<turnstile>expr.Binary bin_op exp1 exp2\<rightarrow>(set_value st2 val)"
+  using BinOp by auto
+lemma [code_pred_intro]:
+"\<lbrakk>st\<turnstile>pexp\<rightarrow>st1;
+             val1 = get_value st1;
+             val = (unary_op_exec un_op val1)\<rbrakk> \<Longrightarrow>
+             st\<turnstile> expr.Unary un_op pexp\<rightarrow>(set_value st1 val)"
+  using UnOp by auto
+lemma [code_pred_intro]:
 "\<lbrakk>val = const_to_basic c\<rbrakk>\<Longrightarrow>
-            st\<turnstile>expr.Const c\<rightarrow>(st,val)"
+              st\<turnstile>expr.Const c\<rightarrow>(set_value st val)"
+  using Const by auto
+lemma [code_pred_intro]:
 "\<lbrakk>val = get_cur_symbvar_by_name st var_name\<rbrakk>\<Longrightarrow>
-           st\<turnstile>expr.SymbolicVar var_name\<rightarrow>(st,val)"
-"\<lbrakk>st\<turnstile>exp\<rightarrow>(st1,pos);
-                 val = get_cur_arvar_by_name_by_pos st var_name pos\<rbrakk>\<Longrightarrow>
-               st\<turnstile>expr.ArrayVar var_name exp\<rightarrow>(st,val)"
+             st\<turnstile>expr.SymbolicVar var_name\<rightarrow>(set_value st val)"
+  using Symbolic by auto
+lemma [code_pred_intro]:
+"\<lbrakk>st\<turnstile>exp\<rightarrow>st1;
+                 pos = get_value st1;
+                 val = get_cur_arvar_by_name_by_pos st1 var_name pos\<rbrakk>\<Longrightarrow>
+                 st\<turnstile>expr.ArrayVar var_name exp\<rightarrow>(set_value st1 val)"
+  using Array by auto
+lemma [code_pred_intro]:
 "\<lbrakk>val = check_proc_status st p_name p_status\<rbrakk>\<Longrightarrow>
-          st\<turnstile>expr.ProcStatEpxr p_name p_status\<rightarrow>(st,val)"
-"\<lbrakk>st\<turnstile>name,as_list\<longrightarrow>(st1,val)\<rbrakk> \<Longrightarrow> st\<turnstile>expr.FunctionCall name as_list \<rightarrow> (st1,val)"
-  by (auto intro: eval_exec_exec_func_assign_param.intros)
+            st\<turnstile>expr.ProcStatEpxr p_name p_status\<rightarrow>(set_value st val)"
+  using PSE by auto
+lemma [code_pred_intro]:
+"\<lbrakk>st\<turnstile>name,as_list\<longrightarrow>st1\<rbrakk> \<Longrightarrow> 
+                 st\<turnstile>expr.FunctionCall name as_list \<rightarrow> st1"
+  using FuncCall by auto
 
-inductive_cases BinOpE[elim!]: "st\<turnstile>expr.Binary bin_op exp1 exp2\<rightarrow>(st2,val)"
-inductive_cases UnOpE[elim!]: "st\<turnstile> expr.Unary un_op pexp\<rightarrow>(st1,val)"
-inductive_cases ConstE[elim!]: "st\<turnstile>expr.Const c\<rightarrow>(st,val)"
-inductive_cases VarE[elim!]: "st\<turnstile>expr.SymbolicVar var_name\<rightarrow>(st,val)"
-inductive_cases ArrayVarE[elim!]: "st\<turnstile>expr.ArrayVar var_name exp\<rightarrow>(st,val)"
-inductive_cases PSE[elim!]: "st\<turnstile>expr.ProcStatEpxr p_name p_status\<rightarrow>(st,val)"
-inductive_cases FuncCallE[elim!]: "st\<turnstile>expr.FunctionCall name as_list \<rightarrow> (st1,val)"
+inductive_cases BinOpE[elim!]: "st\<turnstile>expr.Binary bin_op exp1 exp2\<rightarrow>st3"
+inductive_cases UnOpE[elim!]: "st\<turnstile> expr.Unary un_op pexp\<rightarrow>st2"
+inductive_cases ConstE[elim!]: "st\<turnstile>expr.Const c\<rightarrow>st1"
+inductive_cases SymbolicE[elim!]: "st\<turnstile>expr.SymbolicVar var_name\<rightarrow>st1"
+inductive_cases ArrayE[elim!]: "st\<turnstile>expr.ArrayVar var_name exp\<rightarrow>st2"
+inductive_cases PSE[elim!]: "st\<turnstile>expr.ProcStatEpxr p_name p_status\<rightarrow>st1"
+inductive_cases FuncCallE[elim!]: "st\<turnstile>expr.FunctionCall name as_list \<rightarrow> st1"
 
 text "exec code_pred_intro lemmas"
 lemma [code_pred_intro]:
@@ -169,25 +199,30 @@ lemma [code_pred_intro]:
 "\<lbrakk>st\<turnstile>s1\<longrightarrow>st1;
              st1\<turnstile>s2\<longrightarrow>st2\<rbrakk>\<Longrightarrow>
            st\<turnstile>stmt.Comb s1 s2 \<longrightarrow>st2"
-"\<lbrakk>st\<turnstile>exp\<rightarrow>(st_res,val);
-            (basic_post_type_to_bool val);
-            st\<turnstile>s1\<longrightarrow>st1\<rbrakk>\<Longrightarrow>
-         st\<turnstile>stmt.IfSt exp s1 s2\<longrightarrow>st1"
-"\<lbrakk>st\<turnstile>exp\<rightarrow>(st_res,val);
-           \<not>(basic_post_type_to_bool val);
-           st\<turnstile>s2\<longrightarrow>st1\<rbrakk> \<Longrightarrow> st\<turnstile>stmt.IfSt exp s1 s2\<longrightarrow>st1"
-"\<lbrakk>st\<turnstile>exp\<rightarrow>(st1,val); \<not>(basic_post_type_to_bool val)\<rbrakk>\<Longrightarrow>
-            st\<turnstile>stmt.WhileSt exp s\<longrightarrow>st"
-"\<lbrakk>st\<turnstile>exp\<rightarrow>(st1,val); (basic_post_type_to_bool val);
-              st\<turnstile>s\<longrightarrow>st1;st1\<turnstile>stmt.WhileSt exp s\<longrightarrow>st2\<rbrakk>\<Longrightarrow>
-              st\<turnstile>stmt.WhileSt exp s\<longrightarrow>st2"
-"\<lbrakk>st\<turnstile>exp\<rightarrow>(st1,val);
-                st2 = (set_symbvar st1 var_name val)\<rbrakk>\<Longrightarrow>
-              st\<turnstile>stmt.AssignSt (common_var.Symbolic var_name) exp\<longrightarrow>st2"
-"\<lbrakk>st\<turnstile>exp\<rightarrow>(st1,val1);
-                st1\<turnstile>pos\<rightarrow>(st1,val2);
-                st2 = (set_arvar st1 var_name val2 val1)\<rbrakk>\<Longrightarrow>
-              st\<turnstile>stmt.AssignSt (common_var.Array var_name pos) exp\<longrightarrow>st2"
+"\<lbrakk>st\<turnstile>exp\<rightarrow>st1;
+            (ptype_to_bool (get_value st1));
+            st1\<turnstile>s1\<longrightarrow>st2\<rbrakk>\<Longrightarrow>
+         st\<turnstile>stmt.IfSt exp s1 s2\<longrightarrow>st2"
+"\<lbrakk>st\<turnstile>exp\<rightarrow>st1;
+           \<not>(ptype_to_bool (get_value st1));
+           st1\<turnstile>s2\<longrightarrow>st2\<rbrakk> \<Longrightarrow> st\<turnstile>stmt.IfSt exp s1 s2\<longrightarrow>st2"
+"\<lbrakk>st\<turnstile>exp\<rightarrow>st1; 
+              \<not>(ptype_to_bool (get_value st1))\<rbrakk>\<Longrightarrow>
+              st\<turnstile>stmt.WhileSt exp s\<longrightarrow>st1"
+"\<lbrakk>st\<turnstile>exp\<rightarrow>st1; 
+              (ptype_to_bool (get_value st1));
+              st1\<turnstile>s\<longrightarrow>st2;
+              st2\<turnstile>stmt.WhileSt exp s\<longrightarrow>st3\<rbrakk>\<Longrightarrow>
+              st\<turnstile>stmt.WhileSt exp s\<longrightarrow>st3"
+"\<lbrakk>st\<turnstile>exp\<rightarrow>st1;
+                st2 = (set_cur_symbvar st1 var_name (get_value st1))\<rbrakk>\<Longrightarrow>
+                st\<turnstile>stmt.AssignSt (common_var.Symbolic var_name) exp\<longrightarrow>st2"
+"\<lbrakk>st\<turnstile>exp\<rightarrow>st1;
+                val1 = get_value st1;
+                st1\<turnstile>pos\<rightarrow>st2;
+                val2 = get_value st2;
+                st3 = (set_arvar st2 var_name val2 val1)\<rbrakk>\<Longrightarrow>
+              st\<turnstile>stmt.AssignSt (common_var.Array var_name pos) exp\<longrightarrow>st3"
 "st\<turnstile>stmt.Return\<longrightarrow>st"
 "st\<turnstile>stmt.Exit\<longrightarrow>st"
 "\<lbrakk>st1 = (case stm_name_option of None \<Rightarrow> reset_cur_process st | Some name \<Rightarrow> reset_process st name)\<rbrakk> \<Longrightarrow> 
@@ -201,7 +236,7 @@ lemma [code_pred_intro]:
                       | Some name \<Rightarrow> (set_state st name))\<rbrakk>\<Longrightarrow>
                 st\<turnstile>stmt.SetStateSt st_name_option\<longrightarrow>st1"
 "\<lbrakk>st1 = reset_cur_timer st\<rbrakk> \<Longrightarrow> st\<turnstile>stmt.ResetSt\<longrightarrow>st1"
-  by (auto intro: eval_exec_exec_func_assign_param.intros)
+by (auto intro: eval_exec_exec_func_assign_param.intros)
 
 inductive_cases BlankE[elim!]: "st\<turnstile>stmt.Blank\<longrightarrow>st1"
 thm BlankE
@@ -211,13 +246,35 @@ inductive_cases IfE[elim!]: "st\<turnstile>stmt.IfSt exp s1 s2\<longrightarrow>s
 thm IfE
 inductive_cases LoopE[elim!]: "st\<turnstile>stmt.WhileSt exp s\<longrightarrow>st2"
 thm LoopE
-inductive_cases AssignE[elim!]: "st\<turnstile>stmt.AssignSt v exp\<longrightarrow>st2"
+inductive_cases AssignSE[elim!]: "st\<turnstile>stmt.AssignSt (common_var.Symbolic v) exp\<longrightarrow>st2"
+thm AssignSE
+inductive_cases AssignAE[elim!]: "st\<turnstile>stmt.AssignSt (common_var.Array v exp1) exp2\<longrightarrow>st2"
 inductive_cases ReturnE[elim!]: "st\<turnstile>stmt.Return\<longrightarrow>st"
 inductive_cases ExitE[elim!]: "st\<turnstile>stmt.Exit\<longrightarrow>st"
 inductive_cases ProcessE[elim!]: "st\<turnstile>stmt.ProcessSt p\<longrightarrow>st1"
 inductive_cases SetStateE[elim!]: "st\<turnstile>stmt.SetStateSt st_name_option\<longrightarrow>st1"
 inductive_cases ResetE[elim!]: "st\<turnstile>stmt.ResetSt\<longrightarrow>st1"
 
+text "param_assign code_pred_intro lemmas"
+lemma [code_pred_intro]:
+"assign_param base_st type [] st st"
+"\<lbrakk>base_st \<turnstile> exp \<rightarrow> st;
+                       val = get_value st;
+                       (if as_type = assign_type.ColonEq 
+                        then (assign_param base_st assign_type.ColonEq other (set_cur_symbvar st name val) new_st)
+                        else (assign_param base_st assign_type.ColonEq other st new_st))\<rbrakk> \<Longrightarrow> 
+                      assign_param base_st assign_type.ColonEq ((param_assign.SymbolicVar name as_type exp)#other) st new_st"
+"\<lbrakk>base_st \<turnstile> exp \<rightarrow> st;
+                       val = get_value st;
+                       (if as_type = assign_type.Conseq 
+                        then (assign_param base_st assign_type.Conseq other st new_st) 
+                        else (assign_param base_st assign_type.Conseq other (set_cur_symbvar st name val) new_st))  \<rbrakk> \<Longrightarrow> 
+                      assign_param base_st assign_type.Conseq ((param_assign.SymbolicVar name as_type exp)#other) st new_st"
+  by (auto intro: eval_exec_exec_func_assign_param.intros)
+
+inductive_cases AssignPE[elim!]: "assign_param base_st at pa st new_st"
+
+(*
 text "exec_func code_pred_intro lemmas"
 lemma [code_pred_intro]:
 "\<lbrakk>(f_name,res,vars,stmts) = (get_func_by_name st name);
@@ -226,50 +283,30 @@ lemma [code_pred_intro]:
                   as_proxy_state\<turnstile>stmts\<longrightarrow>st1;
                   assign_param st1 assign_type.Conseq params st new_st;
                   res = (get_cur_symbvar_by_name st1 f_name)\<rbrakk>\<Longrightarrow>
-                st\<turnstile>name,params\<longrightarrow>(new_st,res)"
-  by (auto intro: eval_exec_exec_func_assign_param.FuncStep)
+                st\<turnstile>name,params\<longrightarrow>new_st1"
+  by sledgehammer
 
 inductive_cases FuncE[elim!]:"st\<turnstile>name,params\<longrightarrow>(new_st,res)"
-
-text "param_assign code_pred_intro lemmas"
-lemma [code_pred_intro]:
-"assign_param base_st type [] st st"
-"\<lbrakk>base_st \<turnstile> exp \<rightarrow> (st,val);
-                       (if as_type = assign_type.ColonEq 
-                        then (assign_param base_st assign_type.ColonEq other (set_symbvar st name val) new_st)
-                        else (assign_param base_st assign_type.ColonEq other st new_st))\<rbrakk> \<Longrightarrow> 
-                      assign_param base_st assign_type.ColonEq ((param_assign.SymbolicVar name as_type exp)#other) st new_st"
-"\<lbrakk>base_st \<turnstile> exp \<rightarrow> (st,val);
-                       (if as_type = assign_type.Conseq 
-                        then (assign_param base_st assign_type.Conseq other st new_st) 
-                        else (assign_param base_st assign_type.Conseq other (set_symbvar st name val) new_st))  \<rbrakk> \<Longrightarrow> 
-                      assign_param base_st assign_type.Conseq ((param_assign.SymbolicVar name as_type exp)#other) st new_st"
-  by (auto intro: eval_exec_exec_func_assign_param.intros)
-
-inductive_cases AssignPE[elim!]: "assign_param base_st at pa st new_st"
-
+*)
 inductive 
-  eval_state :: "[model_context,stacked_state,statement_result * model_context] \<Rightarrow> bool" ("_ \<turnstile> _ : _") where
+  eval_state :: "[model_context,stacked_state,model_context] \<Rightarrow> bool" ("_ \<turnstile> _ : _") where
     StateStep : "\<lbrakk>st\<turnstile>stm\<longrightarrow>st1;
                   (case timeout_op of
-                    None \<Rightarrow> (res,st2) = (res,st1)
+                    None \<Rightarrow> st2 = st1
                     | (Some timeout) \<Rightarrow> 
                       (case (extr_timeout_stmt st1 timeout) of 
-                        None \<Rightarrow> (res,st2) = (res,st1)
+                        None \<Rightarrow> st2 = st1
                         | (Some stm1) \<Rightarrow> (st1\<turnstile>stm1\<longrightarrow>st2)))\<rbrakk> \<Longrightarrow> 
-                st \<turnstile>(name,_,stm,timeout_op):(res,st2)"
+                st \<turnstile>(name,stm,timeout_op):st2"
 (*declare eval_state.intros [simp,intro]*)
 
 inductive 
   eval_process :: "[model_context,stacked_process,model_context] \<Rightarrow> bool" ("_\<turnstile>_\<Rightarrow>_") and
   evals_process :: "[model_context,stacked_process list,model_context] \<Rightarrow> bool" ("_\<turnstile>_[\<Rightarrow>]_") where
     ProcStep : "\<lbrakk> new_st = (set_cur_proc_name st name);
-                  new_st\<turnstile>(get_state_by_name state_list (get_cur_proc_state_name new_st)) :(res,st1);
-                  st2 = (case res of 
-                          statement_result.Continue \<Rightarrow> st1
-                        | statement_result.Exit \<Rightarrow> stop_cur_process st1
-                        | statement_result.Return \<Rightarrow> st1);
-                  st3 = (set_into_next_state st2)\<rbrakk> \<Longrightarrow> 
+                  state = (get_state_by_name state_list (get_cur_proc_state_name new_st));
+                  new_st\<turnstile>state:st1;
+                  st3 = (set_into_next_state st1)\<rbrakk> \<Longrightarrow> 
                 st\<turnstile>(name,var_list,state_list) \<Rightarrow> st3"
   | ProcNil : "st\<turnstile>[][\<Rightarrow>]st"
   | ProcCons : "\<lbrakk>active = (is_process_active st (fst pr));
@@ -336,10 +373,12 @@ next
   show "st\<turnstile>(stmt.Comb (stmt.Comb c1 c2) c3)\<longrightarrow>st1" by (simp add: Comb)
 qed
 
+(*
+Doesn't because b may has side effects 
 lemma
-"st\<turnstile>stmt.IfSt b stmt.Blank stmt.Blank \<longrightarrow> st1 \<Longrightarrow> st =st1"
-  by blast
-  
+"st\<turnstile>stmt.IfSt b stmt.Blank stmt.Blank \<longrightarrow> st1 \<Longrightarrow> st = st1"
+  by sledgehammer
+*)  
 
 abbreviation equiv_c :: "stmt \<Rightarrow> stmt \<Rightarrow> bool" (infix "\<sim>" 50) where
 "c \<sim> c' \<equiv> (\<forall>s t. s\<turnstile>c\<longrightarrow>t = s\<turnstile>c'\<longrightarrow>t)"
@@ -378,6 +417,8 @@ proof -
   show ?thesis by meson
 qed
 
+(*
+Doesn't because b may has side effects
 lemma triv_if:
 "st\<turnstile>(stmt.IfSt b c c)\<longrightarrow>st1 \<Longrightarrow> st\<turnstile>c\<longrightarrow>st1"
 proof -
@@ -391,7 +432,7 @@ proof -
     thus ?thesis by blast
   qed
 qed
-
+*)
 (*
 lemma triv_if:
 "(stmt.IfSt b c c) \<sim> c" (is "?w \<sim>?iw")
@@ -434,60 +475,183 @@ proof (induction arbitrary: st2 rule: eval_exec_exec_func_assign_param.induct)
 *)
 
 declare eval_def [simp]
-(*
-code_pred (expected_modes: i \<Rightarrow> i \<Rightarrow> i \<Rightarrow> o)exec_func
-proof - 
-  case exec_func
-  from exec_func.prems show thesis
-  proof (cases)
-    case (FuncStep f_name vars stmts proxy_state as_proxy_state st1)
-    then show ?thesis by (simp add: exec_func.that(1))
-  qed
+
+
+lemma const_simp[simp]: "const_to_basic (const.Nat val) = ptype.Nat val"by auto
+
+lemma value_mirror[simp]: "get_value (set_value st val) = val"
+  apply (induction st)
+  apply auto
+  done
+
+lemma global_vars_mirror1[simp]: "get_global_vars (set_global_vars st vars) = vars"
+  apply (induction st)
+  apply auto
+  done
+
+lemma global_vars_mirror2[simp]:
+  "(get_var_from_global_vars_by_name (set_var_in_global_vars_by_name st name val) name) = val"
+proof -
+  show ?thesis sorry
 qed
 
-code_pred (expected_modes: i \<Rightarrow> i \<Rightarrow> o)eval
+lemma prog_vars_mirror1[simp]: "get_cur_prog_vars (set_cur_prog_vars st vars) = vars" 
 proof -
-  case eval
-  from eval.prems show thesis
-  proof (cases)
-    case (BinOp exp1 st1 val1 exp2 val2 bin_op)
-    from BinOp show thesis by (simp add: eval.that(1))
-  next
-    case (UnOp pexp val1 un_op)
-    from UnOp show thesis by (simp add: eval.that(2))
-  next
-    case (Const c)
-    from Const show thesis by (simp add: eval.that(3))
-  next
-    case (Var var_name)
-    from Var show thesis by (simp add: eval.that(4))
-  next
-    case (PSE p_name p_status)
-    from PSE show thesis by (simp add: eval.that(6))
-  next
-    case (FuncCall name as_list)
-    from FuncCall show thesis by (simp add: eval.that(7))
-  next
-    case (ArrayVar exp uu pos var_name)
-    from ArrayVar  show thesis by (auto simp add: eval.that(5))
-  qed
-  case exec_func
-  from exec_func.prems show thesis
-  proof (cases)
-    case (FuncStep f_name vars stmts proxy_state as_proxy_state st1)
-    then show ?thesis by (simp add: exec_func.that(1))
-  qed
-  
+  show ?thesis sorry
 qed
-  *)
-  
 
-(*
+lemma prog_vars_mirror2[simp]: "(get_prog_var_by_name (set_var_in_prog_vars_by_name st name val) name) = val" 
 proof -
-  case exec
-  from this show thesis by (smt (verit) exec.cases)
+  show ?thesis sorry
 qed
-*)
+
+lemma basic_eq[simp]: "ptype_eq (ptype.Nat v1) (ptype.Nat v2) \<longleftrightarrow> v1 = v2" by auto
+
+declare Let_def[simp] option.split[split]
+
+lemma set_symbvar_global_level_keep[simp]:
+  assumes "get_var_level_by_name st name = var_level.Global"
+  shows "get_var_level_by_name (set_global_var st name val) name = var_level.Global"
+proof -
+  show ?thesis sorry
+qed
+
+lemma set_symbvar_program_level_keep[simp]:
+  assumes "get_var_level_by_name st name = var_level.Program"
+  shows "get_var_level_by_name (set_cur_prog_var st name val) name = var_level.Program"
+proof -
+  show ?thesis sorry
+qed
+
+lemma set_symbvar_process_level_keep[simp]:
+  assumes "get_var_level_by_name st name = var_level.Process"
+  shows "get_var_level_by_name (set_cur_proc_var st name val) name = var_level.Process"
+proof -
+  show ?thesis sorry
+qed
+
+lemma set_symbvar_level_keep[simp]:
+  fixes level :: var_level
+  assumes "get_var_level_by_name st name = level"
+  shows "get_var_level_by_name (set_cur_symbvar st name val) name = level"
+proof (cases level)
+  case Global
+  hence "get_var_level_by_name (set_cur_symbvar st name val) name = get_var_level_by_name (set_global_var st name (stacked_var_init.Symbolic val None)) name" using assms by auto
+  then show ?thesis using set_symbvar_global_level_keep using Global assms by simp
+next
+  case Program
+  hence "get_var_level_by_name (set_cur_symbvar st name val) name = get_var_level_by_name (set_cur_prog_var st name (stacked_var_init.Symbolic val None)) name" using assms by auto
+  then show ?thesis using set_symbvar_program_level_keep using Program assms by simp
+next
+  case Process
+  hence "get_var_level_by_name (set_cur_symbvar st name val) name = get_var_level_by_name (set_cur_proc_var st name (stacked_var_init.Symbolic val None)) name" using assms by auto
+  then show ?thesis using set_symbvar_process_level_keep using Process assms by simp
+qed
+
+lemma global_var_mirror[simp]:
+  assumes "get_var_level_by_name st name = var_level.Global"
+  shows "(get_cur_var_init_by_name (set_global_var st name val) name) = val"
+proof -
+  from assms have 
+   "(get_cur_var_init_by_name (set_global_var st name val) name) = 
+    (get_var_from_global_vars_by_name (get_global_vars 
+      (set_global_var st name val)) 
+    name)" using set_symbvar_global_level_keep by auto
+  hence
+    "(get_cur_var_init_by_name (set_global_var st name val) name) =
+     (get_var_from_global_vars_by_name (get_global_vars 
+      (set_global_vars st (set_var_in_global_vars_by_name (get_global_vars st) name val))) 
+      name)" by simp
+  hence
+    "(get_cur_var_init_by_name (set_global_var st name val) name) =
+     (get_var_from_global_vars_by_name (set_var_in_global_vars_by_name (get_global_vars st) 
+      name val) name)" using global_vars_mirror1 by simp
+  thus ?thesis using global_vars_mirror2 by simp
+qed
+
+lemma program_var_mirror[simp]:
+  assumes "get_var_level_by_name st name = var_level.Program"
+  shows "(get_cur_var_init_by_name (set_cur_prog_var st name val) name) = val"
+proof -
+  from assms have
+  "(get_cur_var_init_by_name (set_cur_prog_var st name val) name) =
+    (get_prog_var_by_name (get_cur_prog_vars 
+    (set_cur_prog_var st name val)) 
+    name)" using set_symbvar_program_level_keep by auto
+  hence "(get_cur_var_init_by_name (set_cur_prog_var st name val) name) =
+          (get_prog_var_by_name (get_cur_prog_vars
+          (set_cur_prog_vars st (set_var_in_prog_vars_by_name (get_cur_prog_vars st) name val))) 
+          name)" by simp
+  hence "(get_cur_var_init_by_name (set_cur_prog_var st name val) name) =
+          (get_prog_var_by_name (set_var_in_prog_vars_by_name (get_cur_prog_vars st) name val)
+          name)" using prog_vars_mirror1 by simp
+  thus ?thesis using prog_vars_mirror2 by simp
+qed
+
+lemma process_var_mirror[simp]:
+  assumes "get_var_level_by_name st name = var_level.Process"
+  shows "(get_cur_var_init_by_name (set_cur_proc_var st name val) name) = val"
+proof -
+  show ?thesis sorry
+qed
+
+lemma symbvar_mirror[simp]:
+  shows "get_cur_symbvar_by_name (set_cur_symbvar st name val) name = val"
+  
+proof (cases "(get_var_level_by_name st name)")
+  case g:Global
+  hence "get_cur_symbvar_by_name (set_cur_symbvar st name val) name = get_cur_symbvar_by_name (set_global_var st name (stacked_var_init.Symbolic val None)) name" by simp
+  from g and this show ?thesis using global_var_mirror by auto
+next
+  case p:Program
+  hence "get_cur_symbvar_by_name (set_cur_symbvar st name val) name = get_cur_symbvar_by_name (set_cur_prog_var st name (stacked_var_init.Symbolic val None)) name" by simp
+  from p and this show ?thesis using program_var_mirror by auto
+next
+  case p:Process
+  hence "get_cur_symbvar_by_name (set_cur_symbvar st name val) name = get_cur_symbvar_by_name (set_cur_proc_var st name (stacked_var_init.Symbolic val None)) name" by simp
+  from p and this show ?thesis using process_var_mirror by auto
+qed
+
+
+declare [[smt_timeout = 1000]]
+
+lemma
+  assumes assms: "st\<turnstile>expr.Const (const.Nat val) \<rightarrow> st_res"
+  shows "st_res = (set_value st (const_to_basic (const.Nat val)))"
+proof -
+  show ?thesis using assms by auto
+qed
+
+
+lemma nat_const_expr[simp]:
+  fixes st st_res :: model_context and name :: string and val :: nat
+  assumes assms: "st\<turnstile>expr.Const (const.Nat val) \<rightarrow> st_res" 
+  shows "(ptype.Nat val) =  (get_value st_res)"
+proof -
+  from assms have "st_res = (set_value st (const_to_basic (const.Nat val)))" using assms by auto
+  hence "get_value st_res = get_value (set_value st (const_to_basic (const.Nat val)))" by simp
+  hence "get_value st_res = (const_to_basic (const.Nat val))" using value_mirror by simp
+  thus ?thesis by simp 
+qed
+  
+(*st\<turnstile>exp\<rightarrow>st1;
+st2 = (set_cur_symbvar st1 var_name (get_value st1))*)
+
+lemma
+  fixes st st_res :: model_context and name :: string and val :: nat
+  assumes assms: "st\<turnstile>stmt.AssignSt (common_var.Symbolic name) (expr.Const (const.Nat val)) \<longrightarrow> st_res" 
+  shows "ptype_eq (get_cur_symbvar_by_name st_res name) (ptype.Nat val)"
+proof -
+  from assms obtain st1 where
+    c1: "st\<turnstile>(expr.Const (const.Nat val))\<rightarrow>st1" and
+    c2: "st_res = (set_cur_symbvar st1 name (get_value st1))" 
+  by (smt (z3) common_var.distinct(1) common_var.inject(1) exec.simps stmt.distinct(11) stmt.distinct(13) stmt.distinct(15) stmt.distinct(17) stmt.distinct(19) stmt.distinct(3) stmt.distinct(5) stmt.distinct(7) stmt.distinct(9) stmt.inject(1))
+  from c1 have "(ptype.Nat val) =  (get_value st1)" by simp
+  from c2 and this have "st_res = (set_cur_symbvar st1 name (ptype.Nat val))" by simp
+  then have "(get_cur_symbvar_by_name st_res name) = (get_cur_symbvar_by_name (set_cur_symbvar st1 name (ptype.Nat val)) name)" by simp
+  then have "(get_cur_symbvar_by_name st_res name) = (ptype.Nat val)" using symbvar_mirror by simp
+  then show "?thesis" using basic_eq by simp
+qed
 
 
 end
