poST_model/poST_function.thy
@@ -7,11 +7,11 @@ datatype func_var =
   OutVar out_var_decl |
   InOutVar inout_var_decl
 type_synonym function_decl = "func_name * 
-                              basic_post_type *
+                              ptype *
                               (func_var list)* 
                               statement_list"
 
 translations
-  (type) "function_decl" <= (type) "func_name * basic_post_type * (func_var list)* statement_list"
+  (type) "function_decl" <= (type) "func_name * ptype * (func_var list)* statement_list"
 
 end
