poST_model/poST_vars.thy
@@ -8,22 +8,22 @@ begin
 datatype array_interval = Expr expr expr | Int int int
 type_synonym array_init = "expr list"
 
-datatype     var_init_decl = Symbolic basic_post_type "expr option" |
-                             Array array_interval "basic_post_type list" "array_init option" |
+datatype     var_init_decl = Symbolic ptype "expr option" |
+                             Array array_interval "ptype list" "array_init option" |
                              FunctionBlock func_block_name
 
 type_synonym in_var_decl = "((symbolic_var * var_init_decl) list)"
 type_synonym out_var_decl = "((symbolic_var * var_init_decl) list)"
 type_synonym inout_var_decl = "((symbolic_var * var_init_decl) list)"
 type_synonym var_decl = "is_const * ((symbolic_var * var_init_decl) list)"
-type_synonym ext_var_decl = "is_const * ((symbolic_var * basic_post_type) list)"
+type_synonym ext_var_decl = "is_const * ((symbolic_var * ptype) list)"
 
 datatype direct_type_perfix = I | Q | M
 datatype direct_size_prefix = X | B | W | D | L
 
 
 type_synonym direct_var = "direct_type_perfix * direct_size_prefix * (int list)"
-type_synonym global_var_init_decl = "direct_var * basic_post_type"
+type_synonym global_var_init_decl = "direct_var * ptype"
 
 datatype all_var_init_decl = Var var_init_decl | GlobalVar global_var_init_decl
 
@@ -34,13 +34,13 @@ type_synonym process_var_decl = "((process_var * process_name) list)"
 
 (*
 translations
-  (type) "array_spec" <= (type) "array_interval * basic_post_type"
+  (type) "array_spec" <= (type) "array_interval * ptype"
   (type) "array_spec_init" <= (type) "array_spec * (array_init option)"
   (type) "var_decl" <= (type) "is_const * (var_init_decl list)"
- (* (type) "ext_var_init_decl" <= (type) "symbolic_var  * basic_post_type"*)
+ (* (type) "ext_var_init_decl" <= (type) "symbolic_var  * ptype"*)
   (type) "ext_var_decl" <= (type) "is_const * (ext_var_init_decl list)"
   (type) "direct_var" <= (type) "direct_type_perfix * direct_size_prefix * (int list)"
- (* (type) "global_var_init_decl" <= (type) "symbolic_var  * direct_var * basic_post_type"*)
+ (* (type) "global_var_init_decl" <= (type) "symbolic_var  * direct_var * ptype"*)
   (type) "global_var_decl" <= (type) "is_const * ((symbolic_var, all_var_init_decl) fmap)"
 *)
 end
