poST_utils/poST_expr_utils.thy
@@ -1,5 +1,5 @@
 theory poST_expr_utils
-  imports basic_poST_types_utils "~~/poST/poST_model/poST_expr"
+  imports ptypes_utils "~~/poST/poST_model/poST_expr"
 begin
 definition proc_status_is :: "proc_status \<Rightarrow> proc_status \<Rightarrow> bool" where
 "proc_status_is s1 s2 = 
@@ -14,28 +14,28 @@ definition proc_status_is :: "proc_status \<Rightarrow> proc_status \<Rightarrow
 declare proc_status_is_def [simp]
 
 text "Executing unary operation"
-definition unary_op_exec :: "unary_op => basic_post_type \<Rightarrow> basic_post_type" where
-"unary_op_exec op var = (case op of unary_op.Not \<Rightarrow> (basic_post_type_not var) | unary_op.Minus \<Rightarrow> (basic_post_type_minus var))"
+definition unary_op_exec :: "unary_op => ptype \<Rightarrow> ptype" where
+"unary_op_exec op var = (case op of unary_op.Not \<Rightarrow> (ptype_not var) | unary_op.Minus \<Rightarrow> (ptype_minus var))"
 declare unary_op_exec_def [simp]
 
 text "Executing binary operation"
-definition binary_op_exec :: "binary_op \<Rightarrow> basic_post_type \<Rightarrow> basic_post_type \<Rightarrow> basic_post_type" where
+definition binary_op_exec :: "binary_op \<Rightarrow> ptype \<Rightarrow> ptype \<Rightarrow> ptype" where
 "binary_op_exec op var1 var2 = 
   (case op of 
-    binary_op.And \<Rightarrow> basic_post_type.Bool(basic_post_type_and var1 var2)|
- binary_op.Or \<Rightarrow> basic_post_type.Bool(basic_post_type_or var1 var2)|
-    binary_op.Xor \<Rightarrow> basic_post_type.Bool(basic_post_type_xor var1 var2) | 
-    binary_op.Eq \<Rightarrow> basic_post_type.Bool(basic_post_type_eq var1 var2)| 
-    binary_op.NotEq \<Rightarrow>basic_post_type.Bool(basic_post_type_noteq var1 var2)| 
-    binary_op.Less \<Rightarrow>basic_post_type.Bool(basic_post_type_less var1 var2)| 
-    binary_op.More \<Rightarrow>basic_post_type.Bool(basic_post_type_more var1 var2)| 
-    binary_op.LessEq \<Rightarrow>basic_post_type.Bool(basic_post_type_lesseq var1 var2)| 
-    binary_op.MoreEq \<Rightarrow>basic_post_type.Bool(basic_post_type_moreeq var1 var2)| 
-    binary_op.Sum \<Rightarrow> basic_post_type_sum var1 var2| 
-    binary_op.Sub \<Rightarrow> basic_post_type_sub var1 var2| 
-    binary_op.Mul \<Rightarrow> basic_post_type_mul var1 var2| 
-    binary_op.Div \<Rightarrow> basic_post_type_div var1 var2| 
-    binary_op.Mod \<Rightarrow> basic_post_type_mod var1 var2)"
+    binary_op.And \<Rightarrow> ptype.Bool(ptype_and var1 var2)|
+ binary_op.Or \<Rightarrow> ptype.Bool(ptype_or var1 var2)|
+    binary_op.Xor \<Rightarrow> ptype.Bool(ptype_xor var1 var2) | 
+    binary_op.Eq \<Rightarrow> ptype.Bool(ptype_eq var1 var2)| 
+    binary_op.NotEq \<Rightarrow>ptype.Bool(ptype_noteq var1 var2)| 
+    binary_op.Less \<Rightarrow>ptype.Bool(ptype_less var1 var2)| 
+    binary_op.More \<Rightarrow>ptype.Bool(ptype_more var1 var2)| 
+    binary_op.LessEq \<Rightarrow>ptype.Bool(ptype_lesseq var1 var2)| 
+    binary_op.MoreEq \<Rightarrow>ptype.Bool(ptype_moreeq var1 var2)| 
+    binary_op.Sum \<Rightarrow> ptype_sum var1 var2| 
+    binary_op.Sub \<Rightarrow> ptype_sub var1 var2| 
+    binary_op.Mul \<Rightarrow> ptype_mul var1 var2| 
+    binary_op.Div \<Rightarrow> ptype_div var1 var2| 
+    binary_op.Mod \<Rightarrow> ptype_mod var1 var2)"
 declare binary_op_exec_def [simp]
 
 end
