poST_utils/ptypes_utils.thy
@@ -1,0 +1,376 @@
+theory ptypes_utils
+  imports "~~/poST/poST_model/ptypes" "~~/poST/poST_utils/bit_types_utils" "~~/poST/poST_utils/poST_time_utils"
+begin
+
+definition const_to_basic :: "const \<Rightarrow> ptype" where
+  "const_to_basic c = (case c of 
+    (const.Nat c) \<Rightarrow> ptype.Nat c |
+    (const.Int c) \<Rightarrow> ptype.Int c |
+    (const.Time c) \<Rightarrow> ptype.Time c |
+    (const.Bool c) \<Rightarrow> ptype.Bool c |
+    (const.Real c) \<Rightarrow> ptype.Real c)"
+declare const_to_basic_def [simp]
+
+definition basic_to_time :: "ptype \<Rightarrow> time" where
+  "basic_to_time c = 
+    (case c of
+      (ptype.Nat v) \<Rightarrow> (nat_to_time v)
+    | (ptype.Int v) \<Rightarrow> (nat_to_time (nat v))
+    | (ptype.Time v) \<Rightarrow> v)"
+declare basic_to_time_def [simp]
+
+definition ptype_to_bptint :: "ptype \<Rightarrow> ptype" where
+  "ptype_to_bptint value = 
+    (case value of 
+      (ptype.Nat val) \<Rightarrow> ptype.Int val |
+      (ptype.Int val) \<Rightarrow> ptype.Int val |
+      (ptype.Real val) \<Rightarrow> ptype.Int (floor val) )"
+declare ptype_to_bptint_def [simp]
+
+definition ptype_to_int :: "ptype \<Rightarrow> int" where
+"ptype_to_int value = 
+    (case value of 
+      (ptype.Nat val) \<Rightarrow> (int val) |
+      (ptype.Int val) \<Rightarrow> val |
+      (ptype.Real val) \<Rightarrow> (floor val) )"
+declare ptype_to_int_def [simp]
+
+definition ptype_to_Bool :: "ptype \<Rightarrow> ptype" where
+"ptype_to_Bool var = (case var of
+  (ptype.Nat val) \<Rightarrow> (ptype.Bool (if val > 0 then True else False)) |
+  (ptype.Int val) \<Rightarrow> (ptype.Bool (if val \<noteq> 0 then True else False)) |
+  (ptype.Real val) \<Rightarrow> (ptype.Bool (if val \<noteq> 0 then True else False)) | 
+  (ptype.Time val) \<Rightarrow> (ptype.Bool (\<not> (time_eq val (time.Time 0 0 0 0 0)))) |
+  (ptype.Bool val) \<Rightarrow> (ptype.Bool val))"
+declare ptype_to_Bool_def [simp]
+
+definition ptype_to_bool :: "ptype \<Rightarrow> bool" where
+"ptype_to_bool var = (case var of
+  (ptype.Nat val) \<Rightarrow>  (if val > 0 then True else False) |
+  (ptype.Int val) \<Rightarrow> (if val \<noteq> 0 then True else False) |
+  (ptype.Real val) \<Rightarrow>  (if val \<noteq> 0 then True else False) | 
+  (ptype.Time val) \<Rightarrow>  (\<not> (time_eq val (time.Time 0 0 0 0 0))) |
+  (ptype.Bool val) \<Rightarrow>  val)"
+declare ptype_to_bool_def [simp]
+
+definition ptype_sum :: "ptype \<Rightarrow> ptype \<Rightarrow> ptype" where
+  "ptype_sum var1 var2 = (case (var1,var2) of
+    ((ptype.Nat var1),(ptype.Nat var2)) \<Rightarrow> ptype.Nat (var1 + var2) |
+    ((ptype.Int var1),(ptype.Int var2)) \<Rightarrow> ptype.Int (var1 + var2) |
+    ((ptype.Real var1),(ptype.Real var2)) \<Rightarrow> ptype.Real (var1 + var2) |
+    ((ptype.Bool var1 ),(ptype.Bool var2)) \<Rightarrow> ptype.Bool (var1 \<or> var2) |
+    ((ptype.Byte var1),(ptype.Byte var2)) \<Rightarrow> ptype.Byte (byte_sum var1 var2) |
+    ((ptype.Time var1),(ptype.Time var2)) \<Rightarrow> ptype.Time (time_sum var1 var2) |
+    ((ptype.Nat var1),(ptype.Int var2)) \<Rightarrow> ptype.Int ((int var1) + var2) | 
+    ((ptype.Int var1),(ptype.Nat var2)) \<Rightarrow> ptype.Int (var1 + (int var2)) |
+    ((ptype.Int var1),(ptype.Real var2)) \<Rightarrow> ptype.Real (var1 + var2) |
+    ((ptype.Real var1),(ptype.Int var2)) \<Rightarrow> ptype.Real (var1 + var2) |
+    ((ptype.Nat var1),(ptype.Real var2)) \<Rightarrow> ptype.Real (var1 + var2) |
+    ((ptype.Real var1),(ptype.Nat var2)) \<Rightarrow> ptype.Real (var1 + var2)) "
+declare ptype_sum_def [simp]
+
+definition const_basic_sum :: "const \<Rightarrow> ptype \<Rightarrow> ptype" where
+  "const_basic_sum c var = ptype_sum (const_to_basic c) var"
+declare const_basic_sum_def [simp]
+
+definition basic_const_sum :: "ptype \<Rightarrow> const \<Rightarrow> ptype" where
+  "basic_const_sum var c = ptype_sum var (const_to_basic c)"
+declare basic_const_sum_def [simp]
+
+(*
+((ptype.Bool var1 ),(ptype.Bool var2)) \<Rightarrow> ptype.Bool (xor var1 var2) |
+((ptype.Time var1),(ptype.Time var2)) \<Rightarrow> ptype.Time (time_sum var1 var2) |
+*)
+definition ptype_sub :: "ptype \<Rightarrow> ptype \<Rightarrow> ptype" where
+  "ptype_sub var1 var2 = (case (var1,var2) of
+    ((ptype.Nat var1),(ptype.Nat var2)) \<Rightarrow> ptype.Nat (var1 - var2) |
+    ((ptype.Int var1),(ptype.Int var2)) \<Rightarrow> ptype.Int (var1 - var2) |
+    ((ptype.Real var1),(ptype.Real var2)) \<Rightarrow> ptype.Real (var1 - var2) |
+    
+    ((ptype.Byte var1),(ptype.Byte var2)) \<Rightarrow> ptype.Byte (byte_sub var1 var2) |
+    
+    ((ptype.Nat var1),(ptype.Int var2)) \<Rightarrow> ptype.Int ((int var1) - var2) | 
+    ((ptype.Int var1),(ptype.Nat var2)) \<Rightarrow> ptype.Int (var1 - (int var2)) |
+    ((ptype.Int var1),(ptype.Real var2)) \<Rightarrow> ptype.Real (var1 - var2) |
+    ((ptype.Real var1),(ptype.Int var2)) \<Rightarrow> ptype.Real (var1 - var2) |
+    ((ptype.Nat var1),(ptype.Real var2)) \<Rightarrow> ptype.Real (var1 - var2) |
+    ((ptype.Real var1),(ptype.Nat var2)) \<Rightarrow> ptype.Real (var1 - var2))"
+declare ptype_sub_def [simp]
+
+definition const_basic_sub :: "const \<Rightarrow> ptype \<Rightarrow> ptype" where
+  "const_basic_sub c var = ptype_sub (const_to_basic c) var"
+declare const_basic_sub_def [simp]
+
+definition basic_const_sub :: "ptype \<Rightarrow> const \<Rightarrow> ptype" where
+  "basic_const_sub var c = ptype_sub var (const_to_basic c)"
+declare basic_const_sub_def [simp]
+
+definition ptype_mul :: "ptype \<Rightarrow> ptype \<Rightarrow> ptype" where
+  "ptype_mul var1 var2 = (case (var1,var2) of
+    ((ptype.Nat var1),(ptype.Nat var2)) \<Rightarrow> ptype.Nat (var1 * var2) |
+    ((ptype.Int var1),(ptype.Int var2)) \<Rightarrow> ptype.Int (var1 * var2) |
+    ((ptype.Real var1),(ptype.Real var2)) \<Rightarrow> ptype.Real (var1 * var2) |
+    
+    ((ptype.Byte var1),(ptype.Byte var2)) \<Rightarrow> ptype.Byte (byte_mul var1 var2) |
+    
+    ((ptype.Nat var1),(ptype.Int var2)) \<Rightarrow> ptype.Int (var1 * var2) | 
+    ((ptype.Int var1),(ptype.Nat var2)) \<Rightarrow> ptype.Int (var1 * var2) |
+    ((ptype.Int var1),(ptype.Real var2)) \<Rightarrow> ptype.Real (var1 * var2) |
+    ((ptype.Real var1),(ptype.Int var2)) \<Rightarrow> ptype.Real (var1 * var2) |
+    ((ptype.Nat var1),(ptype.Real var2)) \<Rightarrow> ptype.Real (var1 * var2) |
+    ((ptype.Real var1),(ptype.Nat var2)) \<Rightarrow> ptype.Real (var1 * var2))"
+declare ptype_mul_def [simp]
+
+definition const_basic_mul :: "const \<Rightarrow> ptype \<Rightarrow> ptype" where
+  "const_basic_mul c var = ptype_mul (const_to_basic c) var"
+declare const_basic_mul_def [simp]
+definition basic_const_mul :: "ptype \<Rightarrow> const \<Rightarrow> ptype" where
+  "basic_const_mul var c = ptype_mul var (const_to_basic c)"
+declare basic_const_mul_def [simp]
+
+definition ptype_div :: "ptype \<Rightarrow> ptype \<Rightarrow> ptype" where
+  "ptype_div var1 var2 = (case (var1,var2) of
+    ((ptype.Nat var1),(ptype.Nat var2)) \<Rightarrow> ptype.Nat (var1 div var2) |
+    ((ptype.Int var1),(ptype.Int var2)) \<Rightarrow> ptype.Int (var1 div var2) |
+    ((ptype.Real var1),(ptype.Real var2)) \<Rightarrow> ptype.Real (var1 div var2) |
+    
+    ((ptype.Byte var1),(ptype.Byte var2)) \<Rightarrow> ptype.Byte (byte_divide var1 var2) |
+    
+    ((ptype.Nat var1),(ptype.Int var2)) \<Rightarrow> ptype.Int (var1 div var2) | 
+    ((ptype.Int var1),(ptype.Nat var2)) \<Rightarrow> ptype.Int (var1 div var2) |
+    ((ptype.Int var1),(ptype.Real var2)) \<Rightarrow> ptype.Real (var1 div var2) |
+    ((ptype.Real var1),(ptype.Int var2)) \<Rightarrow> ptype.Real (var1 div var2) |
+    ((ptype.Nat var1),(ptype.Real var2)) \<Rightarrow> ptype.Real (var1 div var2) |
+    ((ptype.Real var1),(ptype.Nat var2)) \<Rightarrow> ptype.Real (var1 div var2))"
+declare ptype_div_def [simp]
+
+definition const_basic_div :: "const \<Rightarrow> ptype \<Rightarrow> ptype" where
+  "const_basic_div c var = ptype_div (const_to_basic c) var"
+declare const_basic_div_def [simp]
+
+definition basic_const_div :: "ptype \<Rightarrow> const \<Rightarrow> ptype" where
+  "basic_const_div var c = ptype_div var (const_to_basic c)"
+declare basic_const_div_def [simp]
+
+definition ptype_mod :: "ptype \<Rightarrow> ptype \<Rightarrow> ptype" where
+  "ptype_mod var1 var2 = (case (var1,var2) of
+    ((ptype.Nat var1),(ptype.Nat var2)) \<Rightarrow> ptype.Nat (var1 mod var2) |
+    ((ptype.Int var1),(ptype.Int var2)) \<Rightarrow> ptype.Int (var1 mod var2) |
+    
+    ((ptype.Byte var1),(ptype.Byte var2)) \<Rightarrow> ptype.Byte (byte_mod var1 var2) |
+    ((ptype.Nat var1),(ptype.Int var2)) \<Rightarrow> ptype.Int (var1 mod var2) | 
+    ((ptype.Int var1),(ptype.Nat var2)) \<Rightarrow> ptype.Int (var1 mod var2))"
+declare ptype_mod_def [simp]
+
+definition const_basic_mod :: "const \<Rightarrow> ptype \<Rightarrow> ptype" where
+  "const_basic_mod c var = ptype_mod (const_to_basic c) var"
+declare const_basic_mod_def [simp]
+
+definition basic_const_mod :: "ptype \<Rightarrow> const \<Rightarrow> ptype" where
+  "basic_const_mod var c = ptype_mod var (const_to_basic c)"
+declare basic_const_mod_def [simp]
+
+definition ptype_minus :: "ptype \<Rightarrow> ptype" where
+"ptype_minus var = (case var of 
+  (ptype.Int val) \<Rightarrow> (ptype.Int (val * -1)) |
+  (ptype.Real val) \<Rightarrow> (ptype.Real (val * -1)) |
+  (ptype.Bool val) \<Rightarrow> (ptype.Bool (\<not> val)))"
+declare ptype_minus_def [simp]
+
+definition ptype_not:: "ptype \<Rightarrow> ptype" where
+"ptype_not var = (let res = ptype_to_Bool var in
+  (case res of (ptype.Bool val) \<Rightarrow> (ptype.Bool val) ))"
+declare ptype_not_def [simp]
+
+definition ptype_eq :: "ptype \<Rightarrow> ptype \<Rightarrow> bool" where
+  "ptype_eq var1 var2 = (case (var1,var2) of 
+    ((ptype.Nat var1),(ptype.Nat var2)) \<Rightarrow> var1 = var2 |
+    ((ptype.Int var1),(ptype.Int var2)) \<Rightarrow> var1 = var2 |
+    ((ptype.Real var1),(ptype.Real var2)) \<Rightarrow> var1 = var2 |
+    ((ptype.Byte var1),(ptype.Byte var2)) \<Rightarrow> (byte_eq var1 var2) |
+    ((ptype.Time var1),(ptype.Time var2)) \<Rightarrow> (time_eq var1 var2) |
+    ((ptype.Bool var1),(ptype.Bool var2)) \<Rightarrow> var1 = var2 |
+    ((ptype.Nat var1),(ptype.Int var2)) \<Rightarrow> (int var1) = var2 |
+    ((ptype.Int var1),(ptype.Nat var2)) \<Rightarrow> var1 = (int var2) |
+    ((ptype.Nat var1),(ptype.Real var2)) \<Rightarrow> (real var1) = var2 |
+    ((ptype.Real var1),(ptype.Nat var2)) \<Rightarrow> var1 = (real var2) |
+    ((ptype.String var1),(ptype.String var2)) \<Rightarrow> var1 = var2 |
+    (_,_) \<Rightarrow> False )"
+declare ptype_eq_def [simp]
+
+definition const_basic_eq :: "const \<Rightarrow> ptype \<Rightarrow> bool" where 
+"const_basic_eq c var = ptype_eq (const_to_basic c) var"
+declare const_basic_eq_def [simp]
+
+definition basic_const_eq :: "ptype \<Rightarrow> const \<Rightarrow> bool" where 
+"basic_const_eq var c = ptype_eq var (const_to_basic c)"
+declare basic_const_eq_def [simp]
+
+definition ptype_less :: "ptype \<Rightarrow> ptype \<Rightarrow> bool" where
+  "ptype_less var1 var2 = (case (var1,var2) of 
+    ((ptype.Nat var1),(ptype.Nat var2)) \<Rightarrow> var1 < var2 |
+    ((ptype.Int var1),(ptype.Int var2)) \<Rightarrow> var1 < var2 |
+    ((ptype.Real var1),(ptype.Real var2)) \<Rightarrow> var1 < var2 |
+    ((ptype.Byte var1),(ptype.Byte var2)) \<Rightarrow> (byte_less var1 var2) |
+    ((ptype.Time var1),(ptype.Time var2)) \<Rightarrow> (time_less var1 var2) |
+    ((ptype.Bool var1),(ptype.Bool var2)) \<Rightarrow> var1 < var2 |
+    ((ptype.Nat var1),(ptype.Int var2)) \<Rightarrow> (int var1) < var2 |
+    ((ptype.Int var1),(ptype.Nat var2)) \<Rightarrow> var1 < (int var2) |
+    ((ptype.Nat var1),(ptype.Real var2)) \<Rightarrow> var1 < var2 |
+    ((ptype.Real var1),(ptype.Nat var2)) \<Rightarrow> var1 < var2 |
+    ((ptype.Int var1),(ptype.Real var2)) \<Rightarrow> var1 < var2 |
+    ((ptype.Real var1),(ptype.Int var2)) \<Rightarrow> var1 < var2 |
+    (_,_) \<Rightarrow> False )"
+declare ptype_less_def [simp]
+
+definition const_basic_less :: "const \<Rightarrow> ptype \<Rightarrow> bool" where 
+"const_basic_less c var = ptype_less (const_to_basic c) var"
+declare const_basic_less_def [simp]
+
+definition basic_const_less :: "ptype \<Rightarrow> const \<Rightarrow> bool" where 
+"basic_const_less var c = ptype_less var (const_to_basic c)"
+declare basic_const_less_def [simp]
+
+definition ptype_more :: "ptype \<Rightarrow> ptype \<Rightarrow> bool" where
+  "ptype_more var1 var2 = (case (var1,var2) of 
+    ((ptype.Nat var1),(ptype.Nat var2)) \<Rightarrow> var1 > var2 |
+    ((ptype.Int var1),(ptype.Int var2)) \<Rightarrow> var1 > var2 |
+    ((ptype.Real var1),(ptype.Real var2)) \<Rightarrow> var1 > var2 |
+    ((ptype.Byte var1),(ptype.Byte var2)) \<Rightarrow> (byte_more var1 var2) |
+    ((ptype.Time var1),(ptype.Time var2)) \<Rightarrow> (time_more var1 var2) |
+    ((ptype.Bool var1),(ptype.Bool var2)) \<Rightarrow> var1 > var2 |
+    ((ptype.Nat var1),(ptype.Int var2)) \<Rightarrow> (int var1) > var2 |
+    ((ptype.Int var1),(ptype.Nat var2)) \<Rightarrow> var1 > (int var2) |
+    ((ptype.Nat var1),(ptype.Real var2)) \<Rightarrow> var1 > var2 |
+    ((ptype.Real var1),(ptype.Nat var2)) \<Rightarrow> var1 > var2 |
+    ((ptype.Int var1),(ptype.Real var2)) \<Rightarrow> var1 > var2 |
+    ((ptype.Real var1),(ptype.Int var2)) \<Rightarrow> var1 > var2 |
+    (_,_) \<Rightarrow> False )"
+declare ptype_more_def [simp]
+
+definition const_basic_more :: "const \<Rightarrow> ptype \<Rightarrow> bool" where 
+"const_basic_more c var = ptype_more (const_to_basic c) var"
+declare const_basic_more_def [simp]
+
+definition basic_const_more :: "ptype \<Rightarrow> const \<Rightarrow> bool" where 
+"basic_const_more var c = ptype_more var (const_to_basic c)"
+declare basic_const_more_def [simp]
+
+definition ptype_lesseq :: "ptype \<Rightarrow> ptype \<Rightarrow> bool" where
+  "ptype_lesseq var1 var2 = (case (var1,var2) of 
+    ((ptype.Nat var1),(ptype.Nat var2)) \<Rightarrow> var1 \<le> var2 |
+    ((ptype.Int var1),(ptype.Int var2)) \<Rightarrow> var1 \<le> var2 |
+    ((ptype.Real var1),(ptype.Real var2)) \<Rightarrow> var1 \<le> var2 |
+    ((ptype.Byte var1),(ptype.Byte var2)) \<Rightarrow> (byte_eqless var1 var2) |
+    ((ptype.Time var1),(ptype.Time var2)) \<Rightarrow> (time_eqless var1 var2) |
+    ((ptype.Bool var1),(ptype.Bool var2)) \<Rightarrow> var1 \<le> var2 |
+    ((ptype.Nat var1),(ptype.Int var2)) \<Rightarrow> (int var1) \<le> var2 |
+    ((ptype.Int var1),(ptype.Nat var2)) \<Rightarrow> var1 \<le> (int var2) |
+    ((ptype.Nat var1),(ptype.Real var2)) \<Rightarrow> var1 \<le> var2 |
+    ((ptype.Real var1),(ptype.Nat var2)) \<Rightarrow> var1 \<le> var2 |
+    ((ptype.Int var1),(ptype.Real var2)) \<Rightarrow> var1 \<le> var2 |
+    ((ptype.Real var1),(ptype.Int var2)) \<Rightarrow> var1 \<le> var2 |
+    (_,_) \<Rightarrow> False )"
+declare ptype_lesseq_def [simp]
+
+definition const_basic_lesseq :: "const \<Rightarrow> ptype \<Rightarrow> bool" where 
+"const_basic_lesseq c var = ptype_lesseq (const_to_basic c) var"
+declare const_basic_lesseq_def [simp]
+
+definition basic_const_lesseq :: "ptype \<Rightarrow> const \<Rightarrow> bool" where 
+"basic_const_lesseq var c = ptype_lesseq var (const_to_basic c)"
+declare basic_const_lesseq_def [simp]
+
+definition ptype_moreeq :: "ptype \<Rightarrow> ptype \<Rightarrow> bool" where
+  "ptype_moreeq var1 var2 = (case (var1,var2) of 
+    ((ptype.Nat var1),(ptype.Nat var2)) \<Rightarrow> var1 \<ge> var2 |
+    ((ptype.Int var1),(ptype.Int var2)) \<Rightarrow> var1 \<ge> var2 |
+    ((ptype.Real var1),(ptype.Real var2)) \<Rightarrow> var1 \<ge> var2 |
+    ((ptype.Byte var1),(ptype.Byte var2)) \<Rightarrow> (byte_eqmore var1 var2) |
+    ((ptype.Time var1),(ptype.Time var2)) \<Rightarrow> (time_eqmore var1 var2) |
+    ((ptype.Bool var1),(ptype.Bool var2)) \<Rightarrow> var1 \<ge> var2 |
+    ((ptype.Nat var1),(ptype.Int var2)) \<Rightarrow> (int var1) \<ge> var2 |
+    ((ptype.Int var1),(ptype.Nat var2)) \<Rightarrow> var1 \<ge> (int var2) |
+    ((ptype.Nat var1),(ptype.Real var2)) \<Rightarrow> var1 \<ge> var2 |
+    ((ptype.Real var1),(ptype.Nat var2)) \<Rightarrow> var1 \<ge> var2 |
+    ((ptype.Int var1),(ptype.Real var2)) \<Rightarrow> var1 \<ge> var2 |
+    ((ptype.Real var1),(ptype.Int var2)) \<Rightarrow> var1 \<ge> var2 |
+    (_,_) \<Rightarrow> False )"
+declare ptype_moreeq_def [simp]
+
+definition const_basic_moreeq :: "const \<Rightarrow> ptype \<Rightarrow> bool" where 
+"const_basic_moreeq c var = ptype_moreeq (const_to_basic c) var"
+declare const_basic_moreeq_def [simp]
+
+definition basic_const_moreeq :: "ptype \<Rightarrow> const \<Rightarrow> bool" where 
+"basic_const_moreeq var c = ptype_moreeq var (const_to_basic c)"
+declare basic_const_moreeq_def [simp]
+
+definition ptype_noteq :: "ptype \<Rightarrow> ptype \<Rightarrow> bool" where
+  "ptype_noteq var1 var2 = (case (var1,var2) of 
+    ((ptype.Nat var1),(ptype.Nat var2)) \<Rightarrow> var1 \<noteq> var2 |
+    ((ptype.Int var1),(ptype.Int var2)) \<Rightarrow> var1 \<noteq> var2 |
+    ((ptype.Real var1),(ptype.Real var2)) \<Rightarrow> var1 \<noteq> var2 |
+    ((ptype.Byte var1),(ptype.Byte var2)) \<Rightarrow> (byte_noteq var1 var2) |
+    ((ptype.Time var1),(ptype.Time var2)) \<Rightarrow> (time_noteq var1 var2) |
+    ((ptype.Bool var1),(ptype.Bool var2)) \<Rightarrow> var1 \<noteq> var2 |
+    ((ptype.Nat var1),(ptype.Int var2)) \<Rightarrow> (int var1) \<noteq> var2 |
+    ((ptype.Int var1),(ptype.Nat var2)) \<Rightarrow> var1 \<noteq> (int var2) |
+    ((ptype.Nat var1),(ptype.Real var2)) \<Rightarrow> var1 \<noteq> var2 |
+    ((ptype.Real var1),(ptype.Nat var2)) \<Rightarrow> var1 \<noteq> var2 |
+    ((ptype.Int var1),(ptype.Real var2)) \<Rightarrow> var1 \<noteq> var2 |
+    ((ptype.Real var1),(ptype.Int var2)) \<Rightarrow> var1 \<noteq> var2 |
+    (_,_) \<Rightarrow> False )"
+declare ptype_noteq_def [simp]
+
+definition const_basic_noteq :: "const \<Rightarrow> ptype \<Rightarrow> bool" where 
+"const_basic_noteq c var = ptype_noteq (const_to_basic c) var"
+declare const_basic_noteq_def [simp]
+
+definition basic_const_noteq :: "ptype \<Rightarrow> const \<Rightarrow> bool" where 
+"basic_const_noteq var c = ptype_noteq var (const_to_basic c)"
+declare basic_const_noteq_def [simp]
+
+definition ptype_and :: "ptype \<Rightarrow> ptype \<Rightarrow> bool" where
+  "ptype_and var1 var2 = (case (var1,var2) of 
+    ((ptype.Bool var1),(ptype.Bool var2)) \<Rightarrow> var1 \<and> var2 |
+    (_,_) \<Rightarrow> False )"
+declare ptype_and_def [simp]
+
+definition const_basic_and :: "const \<Rightarrow> ptype \<Rightarrow> bool" where 
+"const_basic_and c var = ptype_and (const_to_basic c) var"
+declare const_basic_and_def [simp]
+
+definition basic_const_and :: "ptype \<Rightarrow> const \<Rightarrow> bool" where 
+"basic_const_and var c = ptype_and var (const_to_basic c)"
+declare basic_const_and_def [simp]
+
+definition ptype_or :: "ptype \<Rightarrow> ptype \<Rightarrow> bool" where
+  "ptype_or var1 var2 = (case (var1,var2) of 
+    ((ptype.Bool var1),(ptype.Bool var2)) \<Rightarrow> var1 \<or> var2 |
+    (_,_) \<Rightarrow> False )"
+declare ptype_or_def [simp]
+
+definition const_basic_or :: "const \<Rightarrow> ptype \<Rightarrow> bool" where 
+"const_basic_or c var = ptype_or (const_to_basic c) var"
+declare const_basic_or_def [simp]
+
+definition basic_const_or :: "ptype \<Rightarrow> const \<Rightarrow> bool" where 
+"basic_const_or var c = ptype_or var (const_to_basic c)"
+declare basic_const_or_def [simp]
+
+definition ptype_xor :: "ptype \<Rightarrow> ptype \<Rightarrow> bool" where
+  "ptype_xor var1 var2 = (case (var1,var2) of 
+    ((ptype.Bool var1),(ptype.Bool var2)) \<Rightarrow> var1 \<noteq> var2 |
+    (_,_) \<Rightarrow> False )"
+declare ptype_xor_def [simp]
+
+definition const_basic_xor :: "const \<Rightarrow> ptype \<Rightarrow> bool" where 
+"const_basic_xor c var = ptype_xor (const_to_basic c) var"
+declare const_basic_xor_def [simp]
+
+definition basic_const_xor :: "ptype \<Rightarrow> const \<Rightarrow> bool" where 
+"basic_const_xor var c = ptype_xor var (const_to_basic c)"
+declare basic_const_xor_def [simp]
+
+end
